cogent/isa/ValueSemantics.thy
@@ -16,28 +16,29 @@ begin
 
 
 
-datatype ('f, 'a, 'b) vval = VPrim lit
-                       | VProduct "('f, 'a, 'b) vval" "('f, 'a, 'b) vval"
-                       | VSum name "('f, 'a, 'b) vval"
-                       | VRecord "('f, 'a, 'b) vval list"
+datatype ('f, 'g, 'a, 'b) vval = VPrim lit
+                       | VProduct "('f, 'g, 'a, 'b) vval" "('f, 'g, 'a, 'b) vval"
+                       | VSum name "('f, 'g, 'a, 'b) vval"
+                       | VRecord "('f, 'g, 'a, 'b) vval list"
                        | VAbstract "'a"
                        | VDAbstract "'b"
-                       | VFunction "'f expr" "type list"
+                       | VFunction "('f, 'g) expr" "type list"
                        | VAFunction "'f" "type list"
+                       | VDAFunction "'g" "type list"
                        | VUnit
 
 (* All polymorphic instantiations must have the _same_ value semantics. This means even if the C
 implementations differ they must all refine the same specification *)
-type_synonym ('f, 'a, 'b) vabsfuns = "'f \<Rightarrow> ('f, 'a, 'b) vval \<Rightarrow> ('f, 'a, 'b) vval \<Rightarrow> bool"
+type_synonym ('f, 'g, 'a, 'b) vabsfuns = "'f \<Rightarrow> ('f, 'g, 'a, 'b) vval \<Rightarrow> ('f, 'g, 'a, 'b) vval \<Rightarrow> bool"
+type_synonym ('f, 'g, 'a, 'b) vdabsfuns = "'g \<Rightarrow> ('f, 'g, 'a, 'b) vval \<Rightarrow> ('f, 'g, 'a, 'b) vval \<Rightarrow> bool"
 
-
-definition eval_prim :: "prim_op \<Rightarrow> ('f, 'a, 'b) vval list \<Rightarrow> ('f, 'a, 'b) vval"
+definition eval_prim :: "prim_op \<Rightarrow> ('f, 'g, 'a, 'b) vval list \<Rightarrow> ('f, 'g, 'a, 'b) vval"
 where
   "eval_prim pop xs = VPrim (eval_prim_op pop (map (\<lambda>vv. case vv of VPrim v \<Rightarrow> v | _ \<Rightarrow> LBool False) xs))"
 
 lemma eval_prim_type_change:
-assumes "(eval_prim :: prim_op \<Rightarrow> ('f1, 'a1, 'b1) vval list \<Rightarrow> ('f1, 'a1, 'b1) vval) p (map VPrim lits) = VPrim l"
-shows "(eval_prim :: prim_op \<Rightarrow> ('f2, 'a2, 'b2) vval list \<Rightarrow> ('f2, 'a2, 'b2) vval) p (map VPrim  lits) = VPrim l"
+assumes "(eval_prim :: prim_op \<Rightarrow> ('f1, 'g1, 'a1, 'b1) vval list \<Rightarrow> ('f1, 'g1, 'a1, 'b1) vval) p (map VPrim lits) = VPrim l"
+shows "(eval_prim :: prim_op \<Rightarrow> ('f2, 'g2, 'a2, 'b2) vval list \<Rightarrow> ('f2, 'g2, 'a2, 'b2) vval) p (map VPrim  lits) = VPrim l"
 proof -
 have helper: "(\<lambda>vv. case vv of VPrim v \<Rightarrow> v | _ \<Rightarrow> LBool False) \<circ> VPrim = id" by (rule ext, simp)
 then show ?thesis using assms by (simp add: eval_prim_def helper)
@@ -52,101 +53,108 @@ section {* Semantics *}
 *)
 
 
-inductive v_sem :: "('f, 'a, 'b) vabsfuns \<Rightarrow> ('f, 'a, 'b) vval env \<Rightarrow> 'f expr \<Rightarrow> ('f, 'a, 'b) vval \<Rightarrow> bool"
-          ("_ , _ \<turnstile> _ \<Down> _" [30,0,0,20] 60)
-and       v_sem_all  :: "('f, 'a, 'b) vabsfuns \<Rightarrow> ('f, 'a, 'b) vval list \<Rightarrow> 'f expr list \<Rightarrow> ('f, 'a, 'b) vval list \<Rightarrow> bool"
-          ("_ , _ \<turnstile>* _ \<Down> _" [30,0,0,20] 60)
+inductive v_sem :: "('f, 'g, 'a, 'b) vdabsfuns \<Rightarrow> ('f, 'g, 'a, 'b) vabsfuns \<Rightarrow> ('f, 'g, 'a, 'b) vval env \<Rightarrow> ('f, 'g) expr \<Rightarrow> ('f, 'g, 'a, 'b) vval \<Rightarrow> bool"
+          ("_, _ , _ \<turnstile> _ \<Down> _" [30, 30,0,0,20] 60)
+and       v_sem_all  :: "('f, 'g, 'a, 'b) vdabsfuns \<Rightarrow> ('f, 'g, 'a, 'b) vabsfuns \<Rightarrow> ('f, 'g, 'a, 'b) vval list \<Rightarrow> ('f, 'g) expr list \<Rightarrow> ('f, 'g, 'a, 'b) vval list \<Rightarrow> bool"
+          ("_, _ , _ \<turnstile>* _ \<Down> _" [30, 30,0,0,20] 60)
 where
-  v_sem_var     : "\<xi> , \<gamma> \<turnstile> (Var i) \<Down> (\<gamma> ! i)"
+  v_sem_var     : "\<xi>\<^sub>d , \<xi> , \<gamma> \<turnstile> (Var i) \<Down> (\<gamma> ! i)"
 
-| v_sem_lit     : "\<xi> , \<gamma> \<turnstile> (Lit l) \<Down> VPrim l"
+| v_sem_lit     : "\<xi>\<^sub>d , \<xi> , \<gamma> \<turnstile> (Lit l) \<Down> VPrim l"
 
-| v_sem_prim    : "\<lbrakk> \<xi> , \<gamma> \<turnstile>* as \<Down> as'
-                   \<rbrakk> \<Longrightarrow>  \<xi> , \<gamma> \<turnstile> (Prim p as) \<Down> eval_prim p as'"
+| v_sem_prim    : "\<lbrakk> \<xi>\<^sub>d , \<xi> , \<gamma> \<turnstile>* as \<Down> as'
+                   \<rbrakk> \<Longrightarrow>  \<xi>\<^sub>d , \<xi> , \<gamma> \<turnstile> (Prim p as) \<Down> eval_prim p as'"
 
-| v_sem_fun     : "\<xi> , \<gamma> \<turnstile> Fun f ts \<Down> VFunction f ts"
+| v_sem_fun     : "\<xi>\<^sub>d , \<xi> , \<gamma> \<turnstile> Fun f ts \<Down> VFunction f ts"
 
-| v_sem_afun     : "\<xi> , \<gamma> \<turnstile> AFun f ts \<Down> VAFunction f ts"
+| v_sem_afun     : "\<xi>\<^sub>d , \<xi> , \<gamma> \<turnstile> AFun f ts \<Down> VAFunction f ts"
 
-| v_sem_abs_app : "\<lbrakk> \<xi> , \<gamma> \<turnstile> x \<Down> VAFunction f ts
-                   ; \<xi> , \<gamma> \<turnstile> y \<Down> a
+| v_sem_dafun     : "\<xi>\<^sub>d , \<xi> , \<gamma> \<turnstile> DAFun f ts \<Down> VDAFunction f ts"
+
+| v_sem_abs_app : "\<lbrakk> \<xi>\<^sub>d , \<xi> , \<gamma> \<turnstile> x \<Down> VAFunction f ts
+                   ; \<xi>\<^sub>d , \<xi> , \<gamma> \<turnstile> y \<Down> a
                    ; \<xi> f a r
-                   \<rbrakk> \<Longrightarrow> \<xi> , \<gamma> \<turnstile> (App x y) \<Down> r"
+                   \<rbrakk> \<Longrightarrow> \<xi>\<^sub>d , \<xi> , \<gamma> \<turnstile> (App x y) \<Down> r"
 
-| v_sem_cast    : "\<lbrakk> \<xi> , \<gamma> \<turnstile> e \<Down> VPrim l
+| v_sem_dabs_app : "\<lbrakk> \<xi>\<^sub>d , \<xi> , \<gamma> \<turnstile> x \<Down> VDAFunction g ts
+                   ; \<xi>\<^sub>d , \<xi>, \<gamma> \<turnstile> y \<Down> a
+                   ; \<xi>\<^sub>d g a r
+                   \<rbrakk> \<Longrightarrow> \<xi>\<^sub>d , \<xi> , \<gamma> \<turnstile> (App x y) \<Down> r"
+
+| v_sem_cast    : "\<lbrakk> \<xi>\<^sub>d , \<xi> , \<gamma> \<turnstile> e \<Down> VPrim l
                    ; cast_to \<tau> l = Some l'
-                   \<rbrakk> \<Longrightarrow> \<xi> , \<gamma> \<turnstile> Cast \<tau> e \<Down> VPrim l'"
+                   \<rbrakk> \<Longrightarrow> \<xi>\<^sub>d , \<xi> , \<gamma> \<turnstile> Cast \<tau> e \<Down> VPrim l'"
 
-| v_sem_app     : "\<lbrakk> \<xi> , \<gamma> \<turnstile> x \<Down> VFunction e ts
-                   ; \<xi> , \<gamma> \<turnstile> y \<Down> a
-                   ; \<xi> , [ a ] \<turnstile> specialise ts e \<Down> r
-                   \<rbrakk> \<Longrightarrow> \<xi> , \<gamma> \<turnstile> (App x y) \<Down> r"
+| v_sem_app     : "\<lbrakk> \<xi>\<^sub>d , \<xi> , \<gamma> \<turnstile> x \<Down> VFunction e ts
+                   ; \<xi>\<^sub>d , \<xi> , \<gamma> \<turnstile> y \<Down> a
+                   ; \<xi>\<^sub>d , \<xi> , [ a ] \<turnstile> specialise ts e \<Down> r
+                   \<rbrakk> \<Longrightarrow> \<xi>\<^sub>d , \<xi> , \<gamma> \<turnstile> (App x y) \<Down> r"
 
-| v_sem_con     : "\<lbrakk> \<xi> , \<gamma> \<turnstile> x \<Down> x'
-                   \<rbrakk> \<Longrightarrow> \<xi> , \<gamma> \<turnstile> (Con _ t x) \<Down> VSum t x'"
+| v_sem_con     : "\<lbrakk> \<xi>\<^sub>d , \<xi> , \<gamma> \<turnstile> x \<Down> x'
+                   \<rbrakk> \<Longrightarrow> \<xi>\<^sub>d , \<xi> , \<gamma> \<turnstile> (Con _ t x) \<Down> VSum t x'"
 
-| v_sem_member  : "\<lbrakk> \<xi> , \<gamma> \<turnstile> e \<Down> VRecord fs
-                   \<rbrakk> \<Longrightarrow> \<xi> , \<gamma> \<turnstile> Member e f \<Down> fs ! f"
+| v_sem_member  : "\<lbrakk> \<xi>\<^sub>d , \<xi> , \<gamma> \<turnstile> e \<Down> VRecord fs
+                   \<rbrakk> \<Longrightarrow> \<xi>\<^sub>d , \<xi> , \<gamma> \<turnstile> Member e f \<Down> fs ! f"
 
-| v_sem_unit    : "\<xi> , \<gamma> \<turnstile> Unit \<Down> VUnit"
+| v_sem_unit    : "\<xi>\<^sub>d , \<xi> , \<gamma> \<turnstile> Unit \<Down> VUnit"
 
-| v_sem_tuple   : "\<lbrakk> \<xi> , \<gamma> \<turnstile> x \<Down> x'
-                   ; \<xi> , \<gamma> \<turnstile> y \<Down> y'
-                   \<rbrakk> \<Longrightarrow> \<xi> , \<gamma> \<turnstile> (Tuple x y) \<Down> VProduct x' y'"
+| v_sem_tuple   : "\<lbrakk> \<xi>\<^sub>d , \<xi> , \<gamma> \<turnstile> x \<Down> x'
+                   ; \<xi>\<^sub>d , \<xi> , \<gamma> \<turnstile> y \<Down> y'
+                   \<rbrakk> \<Longrightarrow> \<xi>\<^sub>d , \<xi> , \<gamma> \<turnstile> (Tuple x y) \<Down> VProduct x' y'"
 
-| v_sem_esac    : "\<lbrakk> \<xi> , \<gamma> \<turnstile> t \<Down> VSum ts v
-                   \<rbrakk> \<Longrightarrow> \<xi> , \<gamma> \<turnstile> Esac t ts \<Down> v"
+| v_sem_esac    : "\<lbrakk> \<xi>\<^sub>d , \<xi> , \<gamma> \<turnstile> t \<Down> VSum ts v
+                   \<rbrakk> \<Longrightarrow> \<xi>\<^sub>d , \<xi> , \<gamma> \<turnstile> Esac t ts \<Down> v"
 
-| v_sem_let     : "\<lbrakk> \<xi> , \<gamma> \<turnstile> a \<Down> a'
-                   ; \<xi> , (a' # \<gamma>) \<turnstile> b \<Down> b'
-                   \<rbrakk> \<Longrightarrow> \<xi> , \<gamma> \<turnstile> Let a b \<Down> b'"
+| v_sem_let     : "\<lbrakk> \<xi>\<^sub>d , \<xi> , \<gamma> \<turnstile> a \<Down> a'
+                   ; \<xi>\<^sub>d , \<xi> , (a' # \<gamma>) \<turnstile> b \<Down> b'
+                   \<rbrakk> \<Longrightarrow> \<xi>\<^sub>d , \<xi> , \<gamma> \<turnstile> Let a b \<Down> b'"
 
-| v_sem_letbang : "\<lbrakk> \<xi> , \<gamma> \<turnstile> a \<Down> a'
-                   ; \<xi> , (a' # \<gamma>) \<turnstile> b \<Down> b'
-                   \<rbrakk> \<Longrightarrow> \<xi> , \<gamma> \<turnstile> LetBang vs a b \<Down> b'"
+| v_sem_letbang : "\<lbrakk> \<xi>\<^sub>d , \<xi> , \<gamma> \<turnstile> a \<Down> a'
+                   ; \<xi>\<^sub>d , \<xi> , (a' # \<gamma>) \<turnstile> b \<Down> b'
+                   \<rbrakk> \<Longrightarrow> \<xi>\<^sub>d , \<xi> , \<gamma> \<turnstile> LetBang vs a b \<Down> b'"
 
-| v_sem_case_m  : "\<lbrakk> \<xi> , \<gamma> \<turnstile> x \<Down> VSum t v
-                   ; \<xi> , (v # \<gamma>) \<turnstile> m \<Down> m'
-                   \<rbrakk> \<Longrightarrow> \<xi> , \<gamma> \<turnstile> Case x t m n \<Down> m'"
+| v_sem_case_m  : "\<lbrakk> \<xi>\<^sub>d , \<xi> , \<gamma> \<turnstile> x \<Down> VSum t v
+                   ; \<xi>\<^sub>d , \<xi> , (v # \<gamma>) \<turnstile> m \<Down> m'
+                   \<rbrakk> \<Longrightarrow> \<xi>\<^sub>d , \<xi> , \<gamma> \<turnstile> Case x t m n \<Down> m'"
 
-| v_sem_case_nm : "\<lbrakk> \<xi> , \<gamma> \<turnstile> x \<Down> VSum t' v
+| v_sem_case_nm : "\<lbrakk> \<xi>\<^sub>d , \<xi> , \<gamma> \<turnstile> x \<Down> VSum t' v
                    ; t \<noteq> t'
-                   ; \<xi> , (VSum t' v # \<gamma>) \<turnstile> n \<Down> n'
-                   \<rbrakk> \<Longrightarrow> \<xi> , \<gamma> \<turnstile> Case x t m n \<Down> n'"
+                   ; \<xi>\<^sub>d , \<xi> , (VSum t' v # \<gamma>) \<turnstile> n \<Down> n'
+                   \<rbrakk> \<Longrightarrow> \<xi>\<^sub>d , \<xi> , \<gamma> \<turnstile> Case x t m n \<Down> n'"
 
-| v_sem_if      : "\<lbrakk> \<xi> , \<gamma> \<turnstile> x \<Down> VPrim (LBool b)
-                   ; \<xi> , \<gamma> \<turnstile> if b then t else e \<Down> r
-                   \<rbrakk> \<Longrightarrow> \<xi> , \<gamma> \<turnstile> If x t e \<Down> r"
+| v_sem_if      : "\<lbrakk> \<xi>\<^sub>d , \<xi> , \<gamma> \<turnstile> x \<Down> VPrim (LBool b)
+                   ; \<xi>\<^sub>d , \<xi> , \<gamma> \<turnstile> if b then t else e \<Down> r
+                   \<rbrakk> \<Longrightarrow> \<xi>\<^sub>d , \<xi> , \<gamma> \<turnstile> If x t e \<Down> r"
 
-| v_sem_struct  : "\<lbrakk> \<xi> , \<gamma> \<turnstile>* xs \<Down> vs
-                   \<rbrakk> \<Longrightarrow> \<xi> , \<gamma> \<turnstile> Struct ts xs \<Down> VRecord vs"
+| v_sem_struct  : "\<lbrakk> \<xi>\<^sub>d , \<xi> , \<gamma> \<turnstile>* xs \<Down> vs
+                   \<rbrakk> \<Longrightarrow> \<xi>\<^sub>d , \<xi> , \<gamma> \<turnstile> Struct ts xs \<Down> VRecord vs"
 
-| v_sem_take    : "\<lbrakk> \<xi> , \<gamma> \<turnstile> x \<Down> VRecord fs
-                   ; \<xi> , (fs ! f # VRecord fs # \<gamma>) \<turnstile> e \<Down> e'
-                   \<rbrakk> \<Longrightarrow> \<xi> , \<gamma> \<turnstile> Take x f e \<Down> e'"
+| v_sem_take    : "\<lbrakk> \<xi>\<^sub>d , \<xi> , \<gamma> \<turnstile> x \<Down> VRecord fs
+                   ; \<xi>\<^sub>d , \<xi> , (fs ! f # VRecord fs # \<gamma>) \<turnstile> e \<Down> e'
+                   \<rbrakk> \<Longrightarrow> \<xi>\<^sub>d , \<xi> , \<gamma> \<turnstile> Take x f e \<Down> e'"
 
-| v_sem_put     : "\<lbrakk> \<xi> , \<gamma> \<turnstile> x \<Down> VRecord fs
-                   ; \<xi> , \<gamma> \<turnstile> e \<Down> e'
-                   \<rbrakk> \<Longrightarrow> \<xi> , \<gamma> \<turnstile> Put x f e \<Down> VRecord (fs [ f := e' ])"
+| v_sem_put     : "\<lbrakk> \<xi>\<^sub>d , \<xi> , \<gamma> \<turnstile> x \<Down> VRecord fs
+                   ; \<xi>\<^sub>d , \<xi> , \<gamma> \<turnstile> e \<Down> e'
+                   \<rbrakk> \<Longrightarrow> \<xi>\<^sub>d , \<xi> , \<gamma> \<turnstile> Put x f e \<Down> VRecord (fs [ f := e' ])"
 
-| v_sem_split   : "\<lbrakk> \<xi> , \<gamma> \<turnstile> x \<Down> VProduct a b
-                   ; \<xi> , (a # b # \<gamma>) \<turnstile> e \<Down> e'
-                   \<rbrakk> \<Longrightarrow> \<xi> , \<gamma> \<turnstile> Split x e \<Down> e'"
+| v_sem_split   : "\<lbrakk> \<xi>\<^sub>d , \<xi> , \<gamma> \<turnstile> x \<Down> VProduct a b
+                   ; \<xi>\<^sub>d , \<xi> , (a # b # \<gamma>) \<turnstile> e \<Down> e'
+                   \<rbrakk> \<Longrightarrow> \<xi>\<^sub>d , \<xi> , \<gamma> \<turnstile> Split x e \<Down> e'"
 
-| v_sem_promote : "\<lbrakk> \<xi> , \<gamma> \<turnstile> e \<Down> e'
-                   \<rbrakk> \<Longrightarrow> \<xi> , \<gamma> \<turnstile> Promote t' e \<Down> e'"
+| v_sem_promote : "\<lbrakk> \<xi>\<^sub>d , \<xi> , \<gamma> \<turnstile> e \<Down> e'
+                   \<rbrakk> \<Longrightarrow> \<xi>\<^sub>d , \<xi> , \<gamma> \<turnstile> Promote t' e \<Down> e'"
 
 
-| v_sem_all_empty : "\<xi> , \<gamma> \<turnstile>* [] \<Down> []"
+| v_sem_all_empty : "\<xi>\<^sub>d , \<xi> , \<gamma> \<turnstile>* [] \<Down> []"
 
-| v_sem_all_cons  : "\<lbrakk> \<xi> , \<gamma> \<turnstile> x \<Down> v
-                     ; \<xi> , \<gamma> \<turnstile>* xs \<Down> vs
-                     \<rbrakk> \<Longrightarrow> \<xi> , \<gamma> \<turnstile>* (x # xs) \<Down> (v # vs)"
+| v_sem_all_cons  : "\<lbrakk> \<xi>\<^sub>d , \<xi> , \<gamma> \<turnstile> x \<Down> v
+                     ; \<xi>\<^sub>d , \<xi> , \<gamma> \<turnstile>* xs \<Down> vs
+                     \<rbrakk> \<Longrightarrow> \<xi>\<^sub>d , \<xi> , \<gamma> \<turnstile>* (x # xs) \<Down> (v # vs)"
 
-inductive_cases v_sem_varE  [elim] : "\<xi> , \<gamma> \<turnstile> Var i \<Down> v"
-inductive_cases v_sem_funE  [elim] : "\<xi> , \<gamma> \<turnstile> Fun f ts \<Down> v"
-inductive_cases v_sem_afunE [elim] : "\<xi> , \<gamma> \<turnstile> AFun f ts \<Down> v"
-inductive_cases v_sem_appE  [elim] : "\<xi> , \<gamma> \<turnstile> App a b \<Down> v"
+inductive_cases v_sem_varE  [elim] : "\<xi>\<^sub>d , \<xi> , \<gamma> \<turnstile> Var i \<Down> v"
+inductive_cases v_sem_funE  [elim] : "\<xi>\<^sub>d , \<xi> , \<gamma> \<turnstile> Fun f ts \<Down> v"
+inductive_cases v_sem_afunE [elim] : "\<xi>\<^sub>d , \<xi> , \<gamma> \<turnstile> AFun f ts \<Down> v"
+inductive_cases v_sem_appE  [elim] : "\<xi>\<^sub>d , \<xi> , \<gamma> \<turnstile> App a b \<Down> v"
 
 
 locale value_sem =
@@ -158,40 +166,40 @@ locale value_sem =
 
 context value_sem begin
 
-inductive vval_typing  :: "('f \<Rightarrow> poly_type) \<Rightarrow> ('f, 'a, 'b) vval \<Rightarrow> type \<Rightarrow> bool"
-          ("_ \<turnstile> _ :v _" [30,0,20] 80)
-and vval_typing_record :: "('f \<Rightarrow> poly_type) \<Rightarrow> ('f, 'a, 'b) vval list \<Rightarrow> (name \<times> type \<times> record_state) list \<Rightarrow> bool"
-          ("_ \<turnstile>* _ :vr _" [30,0,20] 80) where
+inductive vval_typing  :: "('g \<Rightarrow> poly_type) \<Rightarrow> ('f \<Rightarrow> poly_type) \<Rightarrow> ('f, 'g, 'a, 'b) vval \<Rightarrow> type \<Rightarrow> bool"
+          ("_, _ \<turnstile> _ :v _" [30,0,20] 80)
+and vval_typing_record :: "('g \<Rightarrow> poly_type) \<Rightarrow> ('f \<Rightarrow> poly_type) \<Rightarrow> ('f, 'g, 'a, 'b) vval list \<Rightarrow> (name \<times> type \<times> record_state) list \<Rightarrow> bool"
+          ("_, _ \<turnstile>* _ :vr _" [30,0,20] 80) where
 
-  v_t_prim     : "\<Xi> \<turnstile> VPrim l :v TPrim (lit_type l)"
+  v_t_prim     : " \<Xi>\<^sub>d, \<Xi> \<turnstile> VPrim l :v TPrim (lit_type l)"
 
-| v_t_product  : "\<lbrakk> \<Xi> \<turnstile> a :v t
-                  ; \<Xi> \<turnstile> b :v u
-                  \<rbrakk> \<Longrightarrow> \<Xi> \<turnstile> VProduct a b :v TProduct t u"
+| v_t_product  : "\<lbrakk>  \<Xi>\<^sub>d, \<Xi> \<turnstile> a :v t
+                  ;  \<Xi>\<^sub>d, \<Xi> \<turnstile> b :v u
+                  \<rbrakk> \<Longrightarrow>  \<Xi>\<^sub>d, \<Xi> \<turnstile> VProduct a b :v TProduct t u"
 
-| v_t_sum      : "\<lbrakk> \<Xi> \<turnstile> a :v t
+| v_t_sum      : "\<lbrakk>  \<Xi>\<^sub>d, \<Xi> \<turnstile> a :v t
                   ; (g, t, Unchecked) \<in> set ts
                   ; distinct (map fst ts)
                   ; [] \<turnstile> TSum ts wellformed
-                  \<rbrakk> \<Longrightarrow> \<Xi> \<turnstile> VSum g a :v TSum ts"
+                  \<rbrakk> \<Longrightarrow>  \<Xi>\<^sub>d, \<Xi> \<turnstile> VSum g a :v TSum ts"
 
-| v_t_record   : "\<lbrakk> \<Xi> \<turnstile>* fs :vr ts
+| v_t_record   : "\<lbrakk>  \<Xi>\<^sub>d, \<Xi> \<turnstile>* fs :vr ts
                   ; distinct (map fst ts)
-                  \<rbrakk> \<Longrightarrow> \<Xi> \<turnstile> VRecord fs :v TRecord ts s"
+                  \<rbrakk> \<Longrightarrow>  \<Xi>\<^sub>d, \<Xi> \<turnstile> VRecord fs :v TRecord ts s"
 
 | v_t_abstract : "\<lbrakk> abs_typing a n ts
                   ; [] \<turnstile>* ts wellformed
-                  \<rbrakk> \<Longrightarrow> \<Xi> \<turnstile> VAbstract a :v TCon n ts s"
+                  \<rbrakk> \<Longrightarrow>  \<Xi>\<^sub>d, \<Xi> \<turnstile> VAbstract a :v TCon n ts s"
 
 | v_t_dabstract : "\<lbrakk> abs_dtyping b n1 n2 n3 ts
                   ; [] \<turnstile>* ts wellformed
-                  \<rbrakk> \<Longrightarrow> \<Xi> \<turnstile> VDAbstract b :v TDCon n1 n2 n3 ts s"
+                  \<rbrakk> \<Longrightarrow>  \<Xi>\<^sub>d, \<Xi> \<turnstile> VDAbstract b :v TDCon n1 n2 n3 ts s"
 
 (*
   The term language type system uses an explicit subtyping rule (Promote), but we want a subtyping-implies-subset relation for values
   so that we can upcast values without having to change their representation. This means we want implicit subsumption for values.
   However, if we introduce a separate subsumption rule for values such as
-  | v_t_subsumption: " \<lbrakk> \<Xi> \<turnstile> v :v t ; [] \<turnstile> t \<sqsubseteq> t' \<rbrakk> \<Longrightarrow> \<Xi> \<turnstile> v :v t' "
+  | v_t_subsumption: " \<lbrakk>  \<Xi>\<^sub>d, \<Xi> \<turnstile> v :v t ; [] \<turnstile> t \<sqsubseteq> t' \<rbrakk> \<Longrightarrow>  \<Xi>\<^sub>d, \<Xi> \<turnstile> v :v t' "
   the canonical forms of values are less obvious.
   Because our definition of subtyping is quite simple, we only really need subsumption for function values.
   So for these two rules, we condense the v_t_subsumption and v_t_afun/v_t_function rules into one.
@@ -201,75 +209,86 @@ and vval_typing_record :: "('f \<Rightarrow> poly_type) \<Rightarrow> ('f, 'a, '
                   ; list_all2 (kinding []) ts ks
                   ; ks \<turnstile> TFun a b wellformed
                   ; [] \<turnstile> TFun (instantiate ts a) (instantiate ts b) \<sqsubseteq> TFun t' u'
-                  \<rbrakk> \<Longrightarrow> \<Xi> \<turnstile> VAFunction f ts :v TFun t' u'"
+                  \<rbrakk> \<Longrightarrow>  \<Xi>\<^sub>d, \<Xi> \<turnstile> VAFunction f ts :v TFun t' u'"
 
-| v_t_function : "\<lbrakk> \<Xi> , K , [ Some t ] \<turnstile> f : u
+| v_t_dafun     : "\<lbrakk> \<Xi>\<^sub>d f = (ks, a, b)
+                  ; list_all2 (kinding []) ts ks
+                  ; ks \<turnstile> TDFun a b wellformed
+                  ; [] \<turnstile> TDFun (instantiate ts a) (instantiate ts b) \<sqsubseteq> TDFun t' u'
+                  \<rbrakk> \<Longrightarrow>  \<Xi>\<^sub>d, \<Xi> \<turnstile> VDAFunction f ts :v TDFun t' u'"
+
+| v_t_function : "\<lbrakk> \<Xi>\<^sub>d, \<Xi> , K , [ Some t ] \<turnstile> f : u
                   ; K \<turnstile> t wellformed
                   ; list_all2 (kinding []) ts K
                   ; [] \<turnstile> TFun (instantiate ts t) (instantiate ts u) \<sqsubseteq> TFun t' u'
-                  \<rbrakk> \<Longrightarrow> \<Xi> \<turnstile> VFunction f ts :v TFun t' u'"
+                  \<rbrakk> \<Longrightarrow>  \<Xi>\<^sub>d, \<Xi> \<turnstile> VFunction f ts :v TFun t' u'"
 
-| v_t_unit     : "\<Xi> \<turnstile> VUnit :v TUnit"
+| v_t_unit     : " \<Xi>\<^sub>d, \<Xi> \<turnstile> VUnit :v TUnit"
 
-| v_t_r_empty  : "\<Xi> \<turnstile>* [] :vr []"
-| v_t_r_cons1  : "\<lbrakk> \<Xi> \<turnstile> x :v t
-                  ; \<Xi> \<turnstile>* xs :vr ts
-                  \<rbrakk> \<Longrightarrow> \<Xi> \<turnstile>* (x # xs) :vr ((n, t, Present) # ts)"
+| v_t_r_empty  : " \<Xi>\<^sub>d, \<Xi> \<turnstile>* [] :vr []"
+| v_t_r_cons1  : "\<lbrakk>  \<Xi>\<^sub>d, \<Xi> \<turnstile> x :v t
+                  ;  \<Xi>\<^sub>d, \<Xi> \<turnstile>* xs :vr ts
+                  \<rbrakk> \<Longrightarrow>  \<Xi>\<^sub>d, \<Xi> \<turnstile>* (x # xs) :vr ((n, t, Present) # ts)"
 | v_t_r_cons2  : "\<lbrakk> [] \<turnstile> t wellformed
-                  ; \<Xi> \<turnstile>* xs :vr ts
-                  \<rbrakk> \<Longrightarrow> \<Xi> \<turnstile>* (x # xs) :vr ((n, t, Taken) # ts)"
+                  ;  \<Xi>\<^sub>d, \<Xi> \<turnstile>* xs :vr ts
+                  \<rbrakk> \<Longrightarrow>  \<Xi>\<^sub>d, \<Xi> \<turnstile>* (x # xs) :vr ((n, t, Taken) # ts)"
 
 
 lemma v_t_prim' [intro]:
 assumes "lit_type l = \<tau>"
-shows   "\<Xi> \<turnstile> VPrim l :v TPrim \<tau>"
+shows   " \<Xi>\<^sub>d, \<Xi> \<turnstile> VPrim l :v TPrim \<tau>"
 using assms by (auto intro: v_t_prim)
 
-inductive_cases v_t_funE      [elim]: "\<Xi> \<turnstile> VFunction f ts :v t"
-inductive_cases v_t_afunE     [elim]: "\<Xi> \<turnstile> VAFunction f ts :v t"
-inductive_cases v_t_recordE   [elim]: "\<Xi> \<turnstile> VRecord fs :v \<tau>"
-inductive_cases v_t_productE  [elim]: "\<Xi> \<turnstile> VProduct a b :v \<tau>"
-inductive_cases v_t_sumE'     [elim]: "\<Xi> \<turnstile> e :v TSum ts"
-inductive_cases v_t_primE     [elim]: "\<Xi> \<turnstile> VPrim l :v TPrim (Num \<tau>)"
+inductive_cases v_t_funE      [elim]: " \<Xi>\<^sub>d, \<Xi> \<turnstile> VFunction f ts :v t"
+inductive_cases v_t_afunE     [elim]: " \<Xi>\<^sub>d, \<Xi> \<turnstile> VAFunction f ts :v t"
+inductive_cases v_t_recordE   [elim]: " \<Xi>\<^sub>d, \<Xi> \<turnstile> VRecord fs :v \<tau>"
+inductive_cases v_t_productE  [elim]: " \<Xi>\<^sub>d, \<Xi> \<turnstile> VProduct a b :v \<tau>"
+inductive_cases v_t_sumE'     [elim]: " \<Xi>\<^sub>d, \<Xi> \<turnstile> e :v TSum ts"
+inductive_cases v_t_primE     [elim]: " \<Xi>\<^sub>d, \<Xi> \<turnstile> VPrim l :v TPrim (Num \<tau>)"
 
-inductive_cases v_t_r_emptyE  [elim]: "\<Xi> \<turnstile>* [] :vr \<tau>s"
-inductive_cases v_t_r_consE   [elim]: "\<Xi> \<turnstile>* (x # xs) :vr \<tau>s"
+inductive_cases v_t_r_emptyE  [elim]: " \<Xi>\<^sub>d, \<Xi> \<turnstile>* [] :vr \<tau>s"
+inductive_cases v_t_r_consE   [elim]: " \<Xi>\<^sub>d, \<Xi> \<turnstile>* (x # xs) :vr \<tau>s"
 
 
-definition vval_typing_all :: "('f \<Rightarrow> poly_type) \<Rightarrow> ('f, 'a, 'b) vval list \<Rightarrow> type list \<Rightarrow> bool"
-           ("_  \<turnstile>* _ :v _" [30,0,20] 80) where
-   "(\<Xi> \<turnstile>* vs :v ts) \<equiv> list_all2 (vval_typing \<Xi>) vs ts"
+definition 
+  vval_typing_all :: "('g \<Rightarrow> poly_type) \<Rightarrow> ('f \<Rightarrow> poly_type) \<Rightarrow> ('f, 'g, 'a, 'b) vval list \<Rightarrow> type list \<Rightarrow> bool"
+           ("_, _  \<turnstile>* _ :v _" [30,0,20] 80) where
+   "(\<Xi>\<^sub>d, \<Xi> \<turnstile>* vs :v ts) \<equiv> list_all2 (vval_typing  \<Xi>\<^sub>d \<Xi>) vs ts"
 
-definition matches :: "('f \<Rightarrow> poly_type) \<Rightarrow>  ('f, 'a, 'b) vval env \<Rightarrow> ctx \<Rightarrow> bool"
-           ("_ \<turnstile> _ matches _" [30,0,20] 60) where
-   "\<Xi> \<turnstile> \<gamma> matches \<Gamma> \<equiv> list_all2 (\<lambda> x m. \<forall> \<tau>. m = Some \<tau> \<longrightarrow> \<Xi> \<turnstile> x :v \<tau>) \<gamma> \<Gamma>"
+definition matches :: "('g \<Rightarrow> poly_type) \<Rightarrow> ('f \<Rightarrow> poly_type) \<Rightarrow>  ('f, 'g, 'a, 'b) vval env \<Rightarrow> ctx \<Rightarrow> bool"
+           ("_, _ \<turnstile> _ matches _" [30,0,20] 60) where
+   "\<Xi>\<^sub>d, \<Xi> \<turnstile> \<gamma> matches \<Gamma> \<equiv> list_all2 (\<lambda> x m. \<forall> \<tau>. m = Some \<tau> \<longrightarrow> \<Xi>\<^sub>d, \<Xi> \<turnstile> x :v \<tau>) \<gamma> \<Gamma>"
 
-lemmas matches_Cons = list_all2_Cons[where P="(\<lambda>x m. \<forall>\<tau>. m = Some \<tau> \<longrightarrow> \<Xi> \<turnstile> x :v \<tau>)" for \<Xi>, simplified matches_def[symmetric]]
+lemmas matches_Cons = 
+  list_all2_Cons[where P="(\<lambda>x m. \<forall>\<tau>. m = Some \<tau> \<longrightarrow> \<Xi>\<^sub>d, \<Xi> \<turnstile> x :v \<tau>)" for \<Xi> \<Xi>\<^sub>d, 
+                 simplified matches_def[symmetric]]
 
-definition proc_env_matches :: "('f \<Rightarrow> ('f, 'a, 'b) vval \<Rightarrow> ('f, 'a, 'b) vval \<Rightarrow> bool) \<Rightarrow> ('f \<Rightarrow> poly_type) \<Rightarrow> bool"
+definition proc_env_matches :: "('f \<Rightarrow> ('f, 'g, 'a, 'b) vval \<Rightarrow> ('f, 'g, 'a, 'b) vval \<Rightarrow> bool) \<Rightarrow> ('f \<Rightarrow> poly_type) \<Rightarrow> bool"
            ("_ matches _" [30,20] 60) where
   "\<xi> matches \<Xi> \<equiv> (\<forall> f. let (K, \<tau>i, \<tau>o) = \<Xi> f
-                        in (\<forall> \<tau>s v v'. list_all2 (kinding []) \<tau>s K
-                                  \<longrightarrow> (\<Xi> \<turnstile> v  :v instantiate \<tau>s \<tau>i)
+                        in (\<forall> \<Xi>\<^sub>d \<tau>s v v'. list_all2 (kinding []) \<tau>s K
+                                  \<longrightarrow> (\<Xi>\<^sub>d , \<Xi> \<turnstile> v  :v instantiate \<tau>s \<tau>i)
                                   \<longrightarrow> \<xi> f v v'
-                                  \<longrightarrow> (\<Xi> \<turnstile> v' :v instantiate \<tau>s \<tau>o)))"
+                                  \<longrightarrow> (\<Xi>\<^sub>d , \<Xi> \<turnstile> v' :v instantiate \<tau>s \<tau>o)))"
 
 
 section {* vval_typing lemmas *}
 
 lemma vval_typing_to_wellformed:
-  shows "\<Xi> \<turnstile> v :v \<tau>     \<Longrightarrow> [] \<turnstile> \<tau> wellformed"
-    and "\<Xi> \<turnstile>* vs :vr fs \<Longrightarrow> [] \<turnstile>* map (fst \<circ> snd) fs wellformed"
+  shows "\<Xi>\<^sub>d , \<Xi> \<turnstile> v :v \<tau>     \<Longrightarrow> [] \<turnstile> \<tau> wellformed"
+    and "\<Xi>\<^sub>d , \<Xi> \<turnstile>* vs :vr fs \<Longrightarrow> [] \<turnstile>* map (fst \<circ> snd) fs wellformed"
 proof (induct rule: vval_typing_vval_typing_record.inducts)
   case v_t_function then show ?case
     by (metis instantiate_wellformed list_all2_kinding_wellformedD subtyping_wellformed_preservation(1) type_wellformed.simps(5) type_wellformed_pretty_def typing_to_wellformed(1))
 next case v_t_afun  then show ?case
     by (metis instantiate_wellformed list_all2_kinding_wellformedD subtyping_wellformed_preservation(1) type_wellformed.simps(5) type_wellformed_pretty_def)
+next case v_t_dafun  then show ?case
+    by (fastforce dest: subtyping_wellformed_preservation(1) list_all2_kinding_wellformedD dest:instantiate_wellformed)
 qed (auto intro: supersumption simp add: list_all_iff kinding_simps dest: kinding_all_record'[simplified o_def])
 
 lemma vval_typing_bang:
-  shows "\<Xi> \<turnstile> x :v \<tau> \<Longrightarrow> \<Xi> \<turnstile> x :v bang \<tau>"
-    and "\<Xi> \<turnstile>* fs :vr \<tau>rs \<Longrightarrow> \<Xi> \<turnstile>* fs :vr map (\<lambda>(n, x, y). (n, bang x, y)) \<tau>rs"
+  shows "\<Xi>\<^sub>d , \<Xi> \<turnstile> x :v \<tau> \<Longrightarrow> \<Xi>\<^sub>d , \<Xi> \<turnstile> x :v bang \<tau>"
+    and "\<Xi>\<^sub>d , \<Xi> \<turnstile>* fs :vr \<tau>rs \<Longrightarrow> \<Xi>\<^sub>d , \<Xi> \<turnstile>* fs :vr map (\<lambda>(n, x, y). (n, bang x, y)) \<tau>rs"
 proof (induct rule: vval_typing_vval_typing_record.inducts)
   case v_t_sum      then show ?case
     by (force simp add: list_all_iff intro: vval_typing_vval_typing_record.intros
@@ -291,16 +310,16 @@ qed (force intro: vval_typing_vval_typing_record.intros)+
 subsection {* vval_typing_record *}
 
 lemma vval_typing_record_length:
-assumes "\<Xi> \<turnstile>* fs :vr \<tau>s"
+assumes "\<Xi>\<^sub>d , \<Xi> \<turnstile>* fs :vr \<tau>s"
 shows   "length fs = length \<tau>s"
 using assms proof (induct fs arbitrary: \<tau>s)
 qed (auto)
 
 lemma vval_typing_record_nth:
-assumes "\<Xi> \<turnstile>* fs :vr \<tau>s"
+assumes "\<Xi>\<^sub>d , \<Xi> \<turnstile>* fs :vr \<tau>s"
 and     "\<tau>s ! f = (n, \<tau>, Present)"
 and     "f < length \<tau>s"
-shows   "\<Xi> \<turnstile> fs ! f :v \<tau>"
+shows   "\<Xi>\<^sub>d , \<Xi> \<turnstile> fs ! f :v \<tau>"
 using assms proof (induct fs arbitrary: f \<tau>s)
      case Nil  then show ?case by (auto)
 next case Cons then show ?case by (case_tac f, auto)
@@ -308,19 +327,19 @@ qed
 
 
 lemma vval_typing_all_record:
-  assumes "\<Xi> \<turnstile>* vs :v ts"
+  assumes "\<Xi>\<^sub>d , \<Xi> \<turnstile>* vs :v ts"
   and "length ns = length ts"
-shows "\<Xi> \<turnstile>* vs :vr zip ns (zip ts (replicate (length ts) Present))"
+shows "\<Xi>\<^sub>d , \<Xi> \<turnstile>* vs :vr zip ns (zip ts (replicate (length ts) Present))"
   using assms[simplified vval_typing_all_def]
   by (induct arbitrary: ns rule: list_all2_induct)
     (auto simp add: length_Suc_conv intro!: vval_typing_vval_typing_record.intros)
 
 lemma vval_typing_record_take:
-  assumes "\<Xi> \<turnstile>* ts :vr \<tau>s"
+  assumes "\<Xi>\<^sub>d , \<Xi> \<turnstile>* ts :vr \<tau>s"
     and "\<tau>s ! f = (n, t, Present)"
     and "[] \<turnstile> t :\<kappa> k"
     and "S \<in> k \<or> taken = Taken"
-  shows "\<Xi> \<turnstile>* ts :vr \<tau>s[ f := (n, t, taken) ]"
+  shows "\<Xi>\<^sub>d , \<Xi> \<turnstile>* ts :vr \<tau>s[ f := (n, t, taken) ]"
   using assms
 proof (induct ts arbitrary: \<tau>s n f)
   case (Cons a ts)
@@ -332,12 +351,12 @@ proof (induct ts arbitrary: \<tau>s n f)
 qed (force intro: vval_typing_vval_typing_record.intros)
 
 lemma vval_typing_record_put:
-assumes "\<Xi> \<turnstile>* ts :vr \<tau>s"
+assumes "\<Xi>\<^sub>d , \<Xi> \<turnstile>* ts :vr \<tau>s"
 and     "\<tau>s ! f = (n, t, taken)"
 and     "[] \<turnstile> t :\<kappa> k"
 and     "D \<in> k \<or> taken = Taken"
-and     "\<Xi> \<turnstile> v :v t"
-shows   "\<Xi> \<turnstile>* ts[ f := v ] :vr \<tau>s[ f := (n, t, Present) ]"
+and     "\<Xi>\<^sub>d , \<Xi> \<turnstile> v :v t"
+shows   "\<Xi>\<^sub>d , \<Xi> \<turnstile>* ts[ f := v ] :vr \<tau>s[ f := (n, t, Present) ]"
 using assms proof (induct ts arbitrary: \<tau>s f)
      case Nil  then show ?case by ( force intro: vval_typing_vval_typing_record.intros)
 next case Cons then show ?case by ( cases taken
@@ -352,22 +371,22 @@ subsection {* Sums and subtyping *}
   (* With the changes to the typing system now, I don't think this holds anymore? ~ v.jackson / 2019.01.10 *)
 lemma width_subtyping:
 assumes "set ts \<subseteq> set us"
-and     "\<Xi> \<turnstile> v :v TSum ts"
+and     "\<Xi>\<^sub>d , \<Xi> \<turnstile> v :v TSum ts"
 and     "[] \<turnstile> TSum us wellformed"
-shows   "\<Xi> \<turnstile> v :v TSum us"
+shows   "\<Xi>\<^sub>d , \<Xi> \<turnstile> v :v TSum us"
 using assms
 by (force simp add: kinding_simps intro: vval_typing_vval_typing_variant_vval_typing_record.intros)
 *)
 lemma sum_downcast:
-  assumes vval_tsum_ts: "\<Xi> \<turnstile> VSum tag v :v TSum ts"
+  assumes vval_tsum_ts: "\<Xi>\<^sub>d , \<Xi> \<turnstile> VSum tag v :v TSum ts"
     and   tag_neq_tag': "tag \<noteq> tag'"
     and   tag'_in_ts  : "(tag', \<tau>, Unchecked) \<in> set ts"
-  shows "\<Xi> \<turnstile> VSum tag v :v TSum (tagged_list_update tag' (\<tau>, Checked) ts)"
+  shows "\<Xi>\<^sub>d , \<Xi> \<turnstile> VSum tag v :v TSum (tagged_list_update tag' (\<tau>, Checked) ts)"
 proof -
   from vval_tsum_ts
   obtain \<tau>1
     where vval_elim_lemmas:
-      "\<Xi> \<turnstile> v :v \<tau>1"
+      "\<Xi>\<^sub>d , \<Xi> \<turnstile> v :v \<tau>1"
       "(tag, \<tau>1, Unchecked) \<in> set ts"
       "distinct (map fst ts)"
       "[] \<turnstile> TSum ts wellformed"
@@ -388,7 +407,7 @@ qed
 
 lemma value_subtyping_to_wellformed:
   "K \<turnstile> t \<sqsubseteq> t'
-  \<Longrightarrow> \<Xi> \<turnstile> v :v t
+  \<Longrightarrow> \<Xi>\<^sub>d , \<Xi> \<turnstile> v :v t
   \<Longrightarrow> K \<turnstile> t' wellformed"
   by (metis instantiate_nothing kinding_iff_wellformed(1) list_all2_Nil substitutivity_single subtyping_wellformed_preservation(1) vval_typing_to_wellformed(1))
 
@@ -428,10 +447,10 @@ proof -
 qed
 
 lemma value_subtyping:
-  shows "\<Xi> \<turnstile> v :v t \<Longrightarrow>[] \<turnstile> t \<sqsubseteq> t' \<Longrightarrow> \<Xi> \<turnstile> v :v t'"
-    and "\<Xi> \<turnstile>* vs :vr ts \<Longrightarrow> [] \<turnstile> TRecord ts s \<sqsubseteq> TRecord ts' s \<Longrightarrow>  \<Xi> \<turnstile>* vs :vr ts'"
+  shows "\<Xi>\<^sub>d , \<Xi> \<turnstile> v :v t \<Longrightarrow>[] \<turnstile> t \<sqsubseteq> t' \<Longrightarrow> \<Xi>\<^sub>d , \<Xi> \<turnstile> v :v t'"
+    and "\<Xi>\<^sub>d , \<Xi> \<turnstile>* vs :vr ts \<Longrightarrow> [] \<turnstile> TRecord ts s \<sqsubseteq> TRecord ts' s \<Longrightarrow>  \<Xi>\<^sub>d , \<Xi> \<turnstile>* vs :vr ts'"
 proof (induct arbitrary: t' and ts' rule: vval_typing_vval_typing_record.inducts)
-  case (v_t_product \<Xi> va ta vb tb)
+  case (v_t_product \<Xi>\<^sub>d \<Xi> va ta vb tb)
   obtain ta' tb' where elims:
     "t' = TProduct ta' tb'"
     "[] \<turnstile> ta \<sqsubseteq> ta'"
@@ -440,7 +459,7 @@ proof (induct arbitrary: t' and ts' rule: vval_typing_vval_typing_record.inducts
   show ?case
     using v_t_product elims by (simp add: vval_typing_vval_typing_record.intros)
 next
-  case (v_t_sum \<Xi> a ta n ts1)
+  case (v_t_sum \<Xi>\<^sub>d  \<Xi> a ta n ts1)
   obtain ts2 where elims:
     "t' = TSum ts2"
     "list_all2 (\<lambda>p1 p2. [] \<turnstile> fst (snd p1) \<sqsubseteq> fst (snd p2)) ts1 ts2"
@@ -481,36 +500,42 @@ next
     using v_t_sum elims n'_in_ts2 n_in_ts_ix subtyping_wellformed_preservation value_sem.v_t_sum value_sem_axioms
     by (metis (no_types, lifting) in_set_conv_nth list_all2_lengthD)
 next
-  case (v_t_record \<Xi> fs ts s)
+  case (v_t_record \<Xi>\<^sub>d \<Xi> fs ts s)
   obtain ts' where elims:
     "t' = TRecord ts' s"
     "distinct (map fst ts')"
     using v_t_record by (auto elim: subtyping.cases intro: vval_typing_vval_typing_record.intros)
 
-  have "\<Xi> \<turnstile>* fs :vr ts'"
-    using elims subty_trecord subtyping_simps(7) v_t_record by presburger
+  have "\<Xi>\<^sub>d , \<Xi> \<turnstile>* fs :vr ts'"
+    using elims subty_trecord subtyping_simps(8) v_t_record by presburger
 
   then show ?case
-    using v_t_record elims  vval_typing_vval_typing_record.intros
-    by blast
+    using v_t_record elims  vval_typing_vval_typing_record.intros 
+    by fast
 next
-  case (v_t_abstract a n ts \<Xi> s)
+  case (v_t_abstract a n ts \<Xi>\<^sub>d \<Xi> s)
   have "t' = TCon n ts s"
     using subtyping.cases v_t_abstract by fastforce
   then show ?case
     using v_t_abstract vval_typing_vval_typing_record.v_t_abstract by blast
 next
-  case (v_t_dabstract a n1 n2 n3 ts \<Xi> s)
+  case (v_t_dabstract a n1 n2 n3 ts \<Xi>\<^sub>d \<Xi> s)
   have "t' = TDCon n1 n2 n3 ts s"
     using subtyping.cases v_t_dabstract by fastforce
   then show ?case
     using v_t_dabstract vval_typing_vval_typing_record.v_t_dabstract by blast
 next
-  case (v_t_afun \<Xi> f ks ta tb ts tfun')
+  case (v_t_afun \<Xi>\<^sub>d \<Xi> f ks ta tb ts tfun')
   then obtain tx ux where "t' = TFun tx ux"
     by (auto elim: subtyping.cases)
   then show ?case
     using v_t_afun by (meson subtyping_trans vval_typing_vval_typing_record.intros)
+next
+  case (v_t_dafun \<Xi>\<^sub>d \<Xi> f ks ta tb ts tfun')
+  then obtain tx ux where "t' = TDFun tx ux"
+    by (auto elim: subtyping.cases)
+  then show ?case
+    using v_t_dafun by (meson subtyping_trans vval_typing_vval_typing_record.intros subtyping_simps)
 next
   case (v_t_function \<Xi> K t f u ts t')
   then obtain tx ux where "t' = TFun tx ux"
@@ -524,14 +549,14 @@ next
   then show ?case
     by (auto elim: subtyping.cases intro: vval_typing_vval_typing_record.intros)
 next
-  case (v_t_r_cons1 \<Xi> x t1 xs ts n)
+  case (v_t_r_cons1 \<Xi>\<^sub>d \<Xi> x t1 xs ts n)
 
   obtain t2 b2 ts2' where field_is: "ts' = (n,t2,b2) # ts2'"
     "([] \<turnstile> t1 \<sqsubseteq> t2)"
     "(if [] \<turnstile> t1 :\<kappa> {D} then Present \<le> b2 else Present = b2)"
     using subtyping_record_cons_split v_t_r_cons1 by blast
 
-  have field_rest: "\<Xi> \<turnstile>* xs :vr ts2'"
+  have field_rest: "\<Xi>\<^sub>d , \<Xi> \<turnstile>* xs :vr ts2'"
     using v_t_r_cons1 field_is subtyping_record_uncons
     by meson
 
@@ -545,14 +570,14 @@ next
     using field_rest field_is v_t_r_cons1 vval_typing_vval_typing_record.v_t_r_cons1 by metis
   qed
 next
-  case (v_t_r_cons2 t1 \<Xi> xs ts x n)
+  case (v_t_r_cons2 t1 \<Xi>\<^sub>d \<Xi> xs ts x n)
 
   obtain t2 b2 ts2' where field_is: "ts' = (n,t2,b2) # ts2'"
     "([] \<turnstile> t1 \<sqsubseteq> t2)"
     "(if [] \<turnstile> t1 :\<kappa> {D} then Taken \<le> b2 else Taken = b2)"
     using subtyping_record_cons_split v_t_r_cons2 by blast
 
-  have field_rest: "\<Xi> \<turnstile>* xs :vr ts2'"
+  have field_rest: "\<Xi>\<^sub>d , \<Xi> \<turnstile>* xs :vr ts2'"
     using v_t_r_cons2 field_is subtyping_record_uncons
     by meson
 
@@ -576,7 +601,7 @@ and     "list_all2 (kinding []) \<delta> K'"
 and     "K \<turnstile> t wellformed"
 and     "K \<turnstile> u wellformed"
 and     "\<Xi> f = (K, t, u)"
-shows   "\<Xi> \<turnstile> VAFunction f (map (instantiate \<delta>) ts) :v TFun (instantiate \<delta> (instantiate ts t))
+shows   "\<Xi>\<^sub>d , \<Xi> \<turnstile> VAFunction f (map (instantiate \<delta>) ts) :v TFun (instantiate \<delta> (instantiate ts t))
                                                            (instantiate \<delta> (instantiate ts u))"
 proof -
   from assms
@@ -598,12 +623,40 @@ proof -
     by (meson list_all2_substitutivity type_wellformed.simps(5) type_wellformed_pretty_def v_t_afun)
 qed
 
+lemma v_t_dafun_instantiate:
+assumes "list_all2 (kinding K') ts K"
+and     "list_all2 (kinding []) \<delta> K'"
+and     "K \<turnstile> t wellformed"
+and     "K \<turnstile> u wellformed"
+and     "\<Xi>\<^sub>d g = (K, t, u)"
+shows   "\<Xi>\<^sub>d , \<Xi> \<turnstile> VDAFunction g (map (instantiate \<delta>) ts) :v TDFun (instantiate \<delta> (instantiate ts t))
+                                                           (instantiate \<delta> (instantiate ts u))"
+proof -
+  from assms
+  have tdfun_eq:
+      "TDFun (instantiate \<delta> (instantiate ts t))
+             (instantiate \<delta> (instantiate ts u))
+      = TDFun (instantiate (map (instantiate \<delta>) ts) t)
+             (instantiate (map (instantiate \<delta>) ts) u)"
+    by (force intro: instantiate_instantiate dest: list_all2_lengthD)
+
+  have tdfun_sub:
+    "[] \<turnstile> TDFun (instantiate (map (instantiate \<delta>) ts) t) (instantiate (map (instantiate \<delta>) ts) u)
+        \<sqsubseteq> TDFun (instantiate       \<delta> (instantiate ts t)) (instantiate       \<delta> (instantiate ts u))"
+    using assms tdfun_eq
+    by (metis subtyping_refl)
+
+  show ?thesis
+    using assms tdfun_sub 
+    by (meson list_all2_substitutivity type_wellformed_pretty_intros(6) v_t_dafun)
+qed
+
 lemma v_t_function_instantiate:
-  assumes "\<Xi>, K, [Some t] \<turnstile> f : u"
+  assumes "\<Xi>\<^sub>d , \<Xi>, K, [Some t] \<turnstile> f : u"
   and     "K \<turnstile> t wellformed"
   and     "list_all2 (kinding []) \<delta> K'"
   assumes "list_all2 (kinding K') ts K"
-  shows   "\<Xi> \<turnstile> VFunction f (map (instantiate \<delta>) ts) :v TFun (instantiate \<delta> (instantiate ts t))
+  shows   "\<Xi>\<^sub>d , \<Xi> \<turnstile> VFunction f (map (instantiate \<delta>) ts) :v TFun (instantiate \<delta> (instantiate ts t))
                                                             (instantiate \<delta> (instantiate ts u))"
 proof -
 from assms have "TFun (instantiate \<delta> (instantiate ts t))
@@ -624,56 +677,58 @@ from assms have "TFun (instantiate \<delta> (instantiate ts t))
     by (meson list_all2_substitutivity type_wellformed.simps(4) type_wellformed_pretty_def v_t_function)
 qed
 
+
 section {* matches lemmas *}
 
 subsection {* matches + context manipulation *}
 lemma matches_split':
 assumes "[] \<turnstile> \<Gamma> \<leadsto> \<Gamma>1 | \<Gamma>2"
-and     "\<Xi> \<turnstile> \<gamma> matches \<Gamma>"
-shows   "\<Xi> \<turnstile> \<gamma> matches \<Gamma>1"
-and     "\<Xi> \<turnstile> \<gamma> matches \<Gamma>2"
+and     "\<Xi>\<^sub>d, \<Xi> \<turnstile> \<gamma> matches \<Gamma>"
+shows   "\<Xi>\<^sub>d, \<Xi> \<turnstile> \<gamma> matches \<Gamma>1"
+and     "\<Xi>\<^sub>d, \<Xi> \<turnstile> \<gamma> matches \<Gamma>2"
 proof -
-  have "\<And>a x y z. [] \<turnstile> x \<leadsto> y \<parallel> z \<Longrightarrow> \<forall>\<tau>. x = Some \<tau> \<longrightarrow> \<Xi> \<turnstile> a :v \<tau> \<Longrightarrow> (\<forall>\<tau>. y = Some \<tau> \<longrightarrow> \<Xi> \<turnstile> a :v \<tau>) \<and> (\<forall>\<tau>. z = Some \<tau> \<longrightarrow> \<Xi> \<turnstile> a :v \<tau>)"
+  have "\<And>a x y z. [] \<turnstile> x \<leadsto> y \<parallel> z \<Longrightarrow> \<forall>\<tau>. x = Some \<tau> \<longrightarrow> \<Xi>\<^sub>d, \<Xi> \<turnstile> a :v \<tau> \<Longrightarrow> 
+              (\<forall>\<tau>. y = Some \<tau> \<longrightarrow> \<Xi>\<^sub>d, \<Xi> \<turnstile> a :v \<tau>) \<and> (\<forall>\<tau>. z = Some \<tau> \<longrightarrow> \<Xi>\<^sub>d, \<Xi> \<turnstile> a :v \<tau>)"
     by (force simp add: split_comp.simps)
-  then show "\<Xi> \<turnstile> \<gamma> matches \<Gamma>1" "\<Xi> \<turnstile> \<gamma> matches \<Gamma>2"
+  then show "\<Xi>\<^sub>d, \<Xi> \<turnstile> \<gamma> matches \<Gamma>1" "\<Xi>\<^sub>d, \<Xi> \<turnstile> \<gamma> matches \<Gamma>2"
     using list_all3_product_over_list_all2
-      [where A="\<lambda>x m. \<forall>\<tau>. m = Some \<tau> \<longrightarrow> \<Xi> \<turnstile> x :v \<tau>" and P="split_comp []",
+      [where A="\<lambda>x m. \<forall>\<tau>. m = Some \<tau> \<longrightarrow> \<Xi>\<^sub>d, \<Xi> \<turnstile> x :v \<tau>" and P="split_comp []",
               simplified matches_def[symmetric] split_def[symmetric]]
     using assms by blast+
 qed
 
 
 lemma matches_split:
-assumes "\<Xi> \<turnstile> \<gamma> matches (instantiate_ctx \<tau>s \<Gamma>)"
+assumes "\<Xi>\<^sub>d, \<Xi> \<turnstile> \<gamma> matches (instantiate_ctx \<tau>s \<Gamma>)"
 and     "list_all2 (kinding []) \<tau>s K"
 and     "K \<turnstile> \<Gamma> \<leadsto> \<Gamma>1 | \<Gamma>2"
-shows   "\<Xi> \<turnstile> \<gamma> matches (instantiate_ctx \<tau>s \<Gamma>1)"
-and     "\<Xi> \<turnstile> \<gamma> matches (instantiate_ctx \<tau>s \<Gamma>2)"
+shows   "\<Xi>\<^sub>d, \<Xi> \<turnstile> \<gamma> matches (instantiate_ctx \<tau>s \<Gamma>1)"
+and     "\<Xi>\<^sub>d, \<Xi> \<turnstile> \<gamma> matches (instantiate_ctx \<tau>s \<Gamma>2)"
 using assms by (auto intro: matches_split' instantiate_ctx_split)
 
 
 lemma matches_split2:
-assumes "\<Xi> \<turnstile> \<gamma> matches (instantiate_ctx \<tau>s \<Gamma>)"
+assumes "\<Xi>\<^sub>d, \<Xi> \<turnstile> \<gamma> matches (instantiate_ctx \<tau>s \<Gamma>)"
 and     "list_all2 (kinding []) \<tau>s K"
 and     "K \<turnstile> \<Gamma> \<leadsto> \<Gamma>1 | \<Gamma>2"
-shows   "(\<Xi> \<turnstile> \<gamma> matches (instantiate_ctx \<tau>s \<Gamma>1)) \<and> (\<Xi> \<turnstile> \<gamma> matches (instantiate_ctx \<tau>s \<Gamma>2))"
+shows   "(\<Xi>\<^sub>d, \<Xi> \<turnstile> \<gamma> matches (instantiate_ctx \<tau>s \<Gamma>1)) \<and> (\<Xi>\<^sub>d, \<Xi> \<turnstile> \<gamma> matches (instantiate_ctx \<tau>s \<Gamma>2))"
 using assms by (auto dest: matches_split)
 
 
 lemma matches_splitE:
-assumes "\<Xi> \<turnstile> \<gamma> matches (instantiate_ctx \<tau>s \<Gamma>)"
+assumes "\<Xi>\<^sub>d, \<Xi> \<turnstile> \<gamma> matches (instantiate_ctx \<tau>s \<Gamma>)"
 and     "list_all2 (kinding []) \<tau>s K"
 and     "K \<turnstile> \<Gamma> \<leadsto> \<Gamma>1 | \<Gamma>2"
-and     "\<lbrakk> \<Xi> \<turnstile> \<gamma> matches (instantiate_ctx \<tau>s \<Gamma>1) ; \<Xi> \<turnstile> \<gamma> matches (instantiate_ctx \<tau>s \<Gamma>2) \<rbrakk> \<Longrightarrow> P"
+and     "\<lbrakk> \<Xi>\<^sub>d, \<Xi> \<turnstile> \<gamma> matches (instantiate_ctx \<tau>s \<Gamma>1) ; \<Xi>\<^sub>d, \<Xi> \<turnstile> \<gamma> matches (instantiate_ctx \<tau>s \<Gamma>2) \<rbrakk> \<Longrightarrow> P"
 shows   "P"
 using assms by (auto dest: matches_split2)
 
 
 lemma matches_split_bang':
 assumes "split_bang [] vs \<Gamma> \<Gamma>1 \<Gamma>2"
-and     "\<Xi> \<turnstile> \<gamma> matches \<Gamma>"
-shows   "\<Xi> \<turnstile> \<gamma> matches \<Gamma>1"
-and     "\<Xi> \<turnstile> \<gamma> matches \<Gamma>2"
+and     "\<Xi>\<^sub>d, \<Xi> \<turnstile> \<gamma> matches \<Gamma>"
+shows   "\<Xi>\<^sub>d, \<Xi> \<turnstile> \<gamma> matches \<Gamma>1"
+and     "\<Xi>\<^sub>d, \<Xi> \<turnstile> \<gamma> matches \<Gamma>2"
   using assms
 proof (induct arbitrary: \<gamma> rule: split_bang.induct)
   case split_bang_empty
@@ -694,17 +749,17 @@ qed
 
 
 lemma matches_split_bang:
-assumes "\<Xi> \<turnstile> \<gamma> matches (instantiate_ctx \<tau>s \<Gamma>)"
+assumes "\<Xi>\<^sub>d, \<Xi> \<turnstile> \<gamma> matches (instantiate_ctx \<tau>s \<Gamma>)"
 and     "list_all2 (kinding []) \<tau>s K"
 and     "split_bang K vs \<Gamma> \<Gamma>1 \<Gamma>2"
-shows   "\<Xi> \<turnstile> \<gamma> matches (instantiate_ctx \<tau>s \<Gamma>1)"
-and     "\<Xi> \<turnstile> \<gamma> matches (instantiate_ctx \<tau>s \<Gamma>2)"
+shows   "\<Xi>\<^sub>d, \<Xi> \<turnstile> \<gamma> matches (instantiate_ctx \<tau>s \<Gamma>1)"
+and     "\<Xi>\<^sub>d, \<Xi> \<turnstile> \<gamma> matches (instantiate_ctx \<tau>s \<Gamma>2)"
 using assms by (auto intro: matches_split_bang' instantiate_ctx_split_bang)
 
 lemma matches_weakening':
-assumes "\<Xi> \<turnstile> \<gamma> matches \<Gamma>"
+assumes "\<Xi>\<^sub>d, \<Xi> \<turnstile> \<gamma> matches \<Gamma>"
 and     "[] \<turnstile> \<Gamma> \<leadsto>w \<Gamma>'"
-shows   "\<Xi> \<turnstile> \<gamma> matches \<Gamma>'"
+shows   "\<Xi>\<^sub>d, \<Xi> \<turnstile> \<gamma> matches \<Gamma>'"
 using assms(2) [simplified weakening_def]
   and assms(1) proof(induct  arbitrary: \<gamma> rule: list_all2_induct)
      case Nil  then show ?case by simp
@@ -714,55 +769,55 @@ next case Cons then show ?case by (force simp:  matches_def
 qed
 
 lemma matches_weakening:
-assumes "\<Xi> \<turnstile> \<gamma> matches (instantiate_ctx \<tau>s \<Gamma>)"
+assumes "\<Xi>\<^sub>d, \<Xi> \<turnstile> \<gamma> matches (instantiate_ctx \<tau>s \<Gamma>)"
 and     "list_all2 (kinding []) \<tau>s K"
 and     "K \<turnstile> \<Gamma> \<leadsto>w \<Gamma>'"
-shows   "\<Xi> \<turnstile> \<gamma> matches (instantiate_ctx \<tau>s \<Gamma>')"
+shows   "\<Xi>\<^sub>d, \<Xi> \<turnstile> \<gamma> matches (instantiate_ctx \<tau>s \<Gamma>')"
 using assms by (auto dest: instantiate_ctx_weaken intro: matches_weakening')
 
 lemma matches_cons':
-assumes "\<Xi> \<turnstile> \<gamma> matches \<Gamma>"
-and     "\<Xi> \<turnstile> x :v \<tau>"
-shows   "\<Xi> \<turnstile> (x # \<gamma>) matches (Some \<tau> # \<Gamma>)"
+assumes "\<Xi>\<^sub>d, \<Xi> \<turnstile> \<gamma> matches \<Gamma>"
+and     "\<Xi>\<^sub>d, \<Xi> \<turnstile> x :v \<tau>"
+shows   "\<Xi>\<^sub>d, \<Xi> \<turnstile> (x # \<gamma>) matches (Some \<tau> # \<Gamma>)"
 using assms by (simp add: matches_def)
 
 lemma matches_cons:
 assumes "list_all2 (kinding []) \<tau>s K"
-and     "\<Xi> \<turnstile> \<gamma> matches (instantiate_ctx \<tau>s \<Gamma>)"
-and     "\<Xi> \<turnstile> x :v instantiate \<tau>s \<tau>"
-shows   "\<Xi> \<turnstile> (x # \<gamma>) matches (instantiate_ctx \<tau>s (Some \<tau> # \<Gamma>))"
+and     "\<Xi>\<^sub>d, \<Xi> \<turnstile> \<gamma> matches (instantiate_ctx \<tau>s \<Gamma>)"
+and     "\<Xi>\<^sub>d, \<Xi> \<turnstile> x :v instantiate \<tau>s \<tau>"
+shows   "\<Xi>\<^sub>d, \<Xi> \<turnstile> (x # \<gamma>) matches (instantiate_ctx \<tau>s (Some \<tau> # \<Gamma>))"
 using assms by (auto intro: matches_cons')
 
 lemma matches_empty':
-shows "\<Xi> \<turnstile> [] matches []"
+shows "\<Xi>\<^sub>d, \<Xi> \<turnstile> [] matches []"
 by (simp add: matches_def)
 
 lemma matches_empty:
-shows "\<Xi> \<turnstile> [] matches instantiate_ctx \<tau>s []"
+shows "\<Xi>\<^sub>d, \<Xi> \<turnstile> [] matches instantiate_ctx \<tau>s []"
 by (simp add: matches_empty' instantiate_ctx_def)
 
 subsection {* other matches properties *}
 
 lemma matches_length:
-assumes "\<Xi> \<turnstile> \<gamma> matches \<Gamma>"
+assumes "\<Xi>\<^sub>d, \<Xi> \<turnstile> \<gamma> matches \<Gamma>"
 shows   "length \<gamma> = length \<Gamma>"
 using assms by (simp add: matches_def list_all2_lengthD)
 
 lemma matches_proj':
-assumes "\<Xi> \<turnstile> \<gamma> matches \<Gamma>"
+assumes "\<Xi>\<^sub>d, \<Xi> \<turnstile> \<gamma> matches \<Gamma>"
 and     "i < length \<Gamma>"
 and     "\<Gamma> ! i = Some \<tau>"
-shows   "\<Xi> \<turnstile> (\<gamma> ! i) :v \<tau>"
+shows   "\<Xi>\<^sub>d, \<Xi> \<turnstile> (\<gamma> ! i) :v \<tau>"
 using assms by (auto dest: list_all2_nthD2
                      simp: matches_def
                      intro: vval_typing_vval_typing_record.intros)
 
 lemma matches_proj:
 assumes "list_all2 (kinding []) \<tau>s K"
-and     "\<Xi> \<turnstile> \<gamma> matches (instantiate_ctx \<tau>s \<Gamma>)"
+and     "\<Xi>\<^sub>d, \<Xi> \<turnstile> \<gamma> matches (instantiate_ctx \<tau>s \<Gamma>)"
 and     "i < length \<Gamma>"
 and     "\<Gamma> ! i = Some \<tau>"
-shows   "\<Xi> \<turnstile> (\<gamma> ! i) :v instantiate \<tau>s \<tau>"
+shows   "\<Xi>\<^sub>d, \<Xi> \<turnstile> (\<gamma> ! i) :v instantiate \<tau>s \<tau>"
 using assms by (auto intro: matches_proj' simp: instantiate_ctx_def)
 
 
@@ -771,9 +826,9 @@ lemma proc_env_matches_abstract:
 assumes "\<xi> matches \<Xi>"
 and     "\<Xi> f = (K, \<tau>i, \<tau>o)"
 and     "list_all2 (kinding []) \<tau>s K"
-and     "\<Xi> \<turnstile> v    :v instantiate \<tau>s \<tau>i"
+and     "\<Xi>\<^sub>d, \<Xi> \<turnstile> v    :v instantiate \<tau>s \<tau>i"
 and     "\<xi> f v v'"
-shows   "\<Xi> \<turnstile> v' :v instantiate \<tau>s \<tau>o"
+shows   "\<Xi>\<^sub>d, \<Xi> \<turnstile> v' :v instantiate \<tau>s \<tau>o"
 using assms by ( clarsimp simp: proc_env_matches_def
                , drule_tac x = f in spec
                , auto)
@@ -782,15 +837,15 @@ using assms by ( clarsimp simp: proc_env_matches_def
 section {* Type Safety *}
 
 theorem progress:
-assumes "\<Xi>, K, \<Gamma> \<turnstile> e : \<tau>"
+assumes "\<Xi>\<^sub>d, \<Xi>, K, \<Gamma> \<turnstile> e : \<tau>"
 and     "\<xi> matches \<Xi>"
 and     "list_all2 (kinding []) \<tau>s K"
-and     "\<Xi> \<turnstile> \<gamma> matches (instantiate_ctx \<tau>s \<Gamma>)"
-shows   "\<exists>! v. \<xi>, \<gamma> \<turnstile> specialise \<tau>s e \<Down> v"
+and     "\<Xi>\<^sub>d, \<Xi> \<turnstile> \<gamma> matches (instantiate_ctx \<tau>s \<Gamma>)"
+shows   "\<exists>! v. \<xi>\<^sub>d, \<xi>, \<gamma> \<turnstile> specialise \<tau>s e \<Down> v"
 oops
 
 lemma v_t_map_TPrimD:
-  "\<Xi> \<turnstile>* vs :v map TPrim \<tau>s
+  "\<Xi>\<^sub>d, \<Xi> \<turnstile>* vs :v map TPrim \<tau>s
     \<Longrightarrow> \<exists>lits. vs = map VPrim lits \<and> map lit_type lits = \<tau>s"
   unfolding vval_typing_all_def list_all2_map2
 proof (induct rule: list_all2_induct)
@@ -809,18 +864,18 @@ qed auto
 
 lemma eval_prim_preservation:
 assumes "prim_op_type p = (\<tau>s, \<tau>)"
-and     "\<Xi> \<turnstile>* vs :v map TPrim \<tau>s"
-shows   "\<Xi> \<turnstile>  eval_prim p vs :v TPrim \<tau>"
+and     "\<Xi>\<^sub>d, \<Xi> \<turnstile>* vs :v map TPrim \<tau>s"
+shows   "\<Xi>\<^sub>d, \<Xi> \<turnstile>  eval_prim p vs :v TPrim \<tau>"
 using assms v_t_prim[where \<Xi>=\<Xi> and l="case eval_prim p vs of VPrim v \<Rightarrow> v"]
 by (clarsimp simp add: eval_prim_def o_def eval_prim_op_lit_type dest!: v_t_map_TPrimD)
 
 theorem preservation:
 assumes "list_all2 (kinding []) \<tau>s K"
 and     "proc_ctx_wellformed \<Xi>"
-and     "\<Xi> \<turnstile> \<gamma> matches (instantiate_ctx \<tau>s \<Gamma>)"
+and     "\<Xi>\<^sub>d, \<Xi> \<turnstile> \<gamma> matches (instantiate_ctx \<tau>s \<Gamma>)"
 and     "\<xi> matches \<Xi>"
-shows   "\<lbrakk> \<xi>, \<gamma> \<turnstile>  specialise \<tau>s e \<Down> v  ; \<Xi>, K, \<Gamma> \<turnstile>  e  : \<tau> \<rbrakk> \<Longrightarrow>  \<Xi> \<turnstile>  v  :v instantiate \<tau>s \<tau>"
-and     "\<lbrakk> \<xi>, \<gamma> \<turnstile>* map (specialise \<tau>s) es \<Down> vs ; \<Xi>, K, \<Gamma> \<turnstile>* es : \<tau>s' \<rbrakk> \<Longrightarrow> \<Xi> \<turnstile>* vs :v map (instantiate \<tau>s) \<tau>s'"
+shows   "\<lbrakk> \<xi>\<^sub>d, \<xi>, \<gamma> \<turnstile>  specialise \<tau>s e \<Down> v  ; \<Xi>\<^sub>d, \<Xi>, K, \<Gamma> \<turnstile>  e  : \<tau> \<rbrakk> \<Longrightarrow>  \<Xi>\<^sub>d, \<Xi> \<turnstile>  v  :v instantiate \<tau>s \<tau>"
+and     "\<lbrakk> \<xi>\<^sub>d, \<xi>, \<gamma> \<turnstile>* map (specialise \<tau>s) es \<Down> vs ; \<Xi>\<^sub>d, \<Xi>, K, \<Gamma> \<turnstile>* es : \<tau>s' \<rbrakk> \<Longrightarrow> \<Xi>\<^sub>d, \<Xi> \<turnstile>* vs :v map (instantiate \<tau>s) \<tau>s'"
 using assms proof (induct "specialise \<tau>s e"        v
                       and "map (specialise \<tau>s) es" vs
                       arbitrary: e  \<tau>s K \<tau>   \<Gamma>
@@ -838,9 +893,11 @@ next case v_sem_cast    then show ?case by ( case_tac e, simp_all
                                            , fastforce elim!: upcast_valid_cast_to)
 next case v_sem_afun    then show ?case by ( case_tac e, simp_all
                                            , fastforce intro: v_t_afun_instantiate simp add: kinding_simps)
+next case v_sem_dafun    then show ?case by ( case_tac e, simp_all
+                                           , fastforce intro: v_t_dafun_instantiate simp add: kinding_simps)
 next case v_sem_fun     then show ?case by ( case_tac e, simp_all
                                            , fastforce intro: v_t_function_instantiate)
-next case (v_sem_con \<xi> \<gamma> x_spec x' ts_inst tag)
+next case (v_sem_con \<xi>\<^sub>d \<xi> \<gamma> x_spec x' ts_inst tag)
   then show ?case
   proof (cases e)
     case (Con ts tag' x)
@@ -855,13 +912,13 @@ next case (v_sem_con \<xi> \<gamma> x_spec x' ts_inst tag)
     moreover then obtain t
       where con_elims:
         "\<tau> = TSum ts"
-        "\<Xi>, K, \<Gamma> \<turnstile> x : t"
+        "\<Xi>\<^sub>d, \<Xi>, K, \<Gamma> \<turnstile> x : t"
         "distinct (map fst ts)"
         "K \<turnstile> TSum ts wellformed"
         "(tag, t, Unchecked) \<in> set ts"
       using Con v_sem_con.prems
       by auto
-    ultimately have "\<Xi> \<turnstile> VSum tag x' :v TSum (map (\<lambda>(c, t, b). (c, instantiate \<tau>s t, b)) ts)"
+    ultimately have "\<Xi>\<^sub>d, \<Xi> \<turnstile> VSum tag x' :v TSum (map (\<lambda>(c, t, b). (c, instantiate \<tau>s t, b)) ts)"
       using v_sem_con.hyps(2) v_sem_con.prems con_elims typing_simps
     proof (intro v_t_sum)
       show "(tag, instantiate \<tau>s t, Unchecked) \<in> set (map (\<lambda>(c, t, b). (c, instantiate \<tau>s t, b)) ts)"
@@ -869,7 +926,7 @@ next case (v_sem_con \<xi> \<gamma> x_spec x' ts_inst tag)
     next
       show "[] \<turnstile> TSum (map (\<lambda>(c, t, b). (c, instantiate \<tau>s t, b)) ts) wellformed"
         using con_elims v_sem_con.prems
-        by (metis instantiate.simps(7) kinding_iff_wellformed(1) substitutivity_single)
+        by (metis instantiate.simps(8) kinding_iff_wellformed(1) substitutivity_single)
     qed auto
     then show ?thesis
       using con_elims by auto
@@ -885,7 +942,7 @@ next case v_sem_case_m  then show ?case by ( case_tac e, simp_all
                                            , fastforce intro: matches_split
                                                               matches_cons [simplified]
                                                        dest:  distinct_fst)
-next case (v_sem_case_nm \<xi> \<gamma> x tag' v tag n n' m)
+next case (v_sem_case_nm \<xi>\<^sub>d  \<xi> \<gamma> x tag' v tag n n' m)
   from v_sem_case_nm.hyps(6)
   show ?case
   proof (case_tac e; clarsimp)
@@ -897,34 +954,34 @@ next case (v_sem_case_nm \<xi> \<gamma> x tag' v tag n n' m)
 
     then obtain \<Gamma>1 \<Gamma>2 ts ta
       where split\<Gamma>: "K \<turnstile> \<Gamma> \<leadsto> \<Gamma>1 | \<Gamma>2"
-      and typing_x1: "\<Xi>, K, \<Gamma>1 \<turnstile> x1 : TSum ts"
+      and typing_x1: "\<Xi>\<^sub>d, \<Xi>, K, \<Gamma>1 \<turnstile> x1 : TSum ts"
       and ta_in_ts: "(tag, ta, Unchecked) \<in> set ts"
-      and typing_x3: "\<Xi>, K, Some ta # \<Gamma>2 \<turnstile> x3 : \<tau>"
-      and typing_x4: "\<Xi>, K, Some (TSum (tagged_list_update tag (ta, Checked) ts)) # \<Gamma>2 \<turnstile> x4 : \<tau>"
+      and typing_x3: "\<Xi>\<^sub>d, \<Xi>, K, Some ta # \<Gamma>2 \<turnstile> x3 : \<tau>"
+      and typing_x4: "\<Xi>\<^sub>d, \<Xi>, K, Some (TSum (tagged_list_update tag (ta, Checked) ts)) # \<Gamma>2 \<turnstile> x4 : \<tau>"
       using v_sem_case_nm.prems
       by fastforce
 
     from split\<Gamma>
-    have \<gamma>_matches_\<Gamma>1: "\<Xi> \<turnstile> \<gamma> matches instantiate_ctx \<tau>s \<Gamma>1"
-      and \<gamma>_matches_\<Gamma>2: "\<Xi> \<turnstile> \<gamma> matches instantiate_ctx \<tau>s \<Gamma>2"
+    have \<gamma>_matches_\<Gamma>1: "\<Xi>\<^sub>d, \<Xi> \<turnstile> \<gamma> matches instantiate_ctx \<tau>s \<Gamma>1"
+      and \<gamma>_matches_\<Gamma>2: "\<Xi>\<^sub>d, \<Xi> \<turnstile> \<gamma> matches instantiate_ctx \<tau>s \<Gamma>2"
       using matches_split2 v_sem_case_nm.prems
       by fastforce+
 
-    have "\<Xi> \<turnstile> VSum tag' v :v instantiate \<tau>s (TSum ts)"
+    have "\<Xi>\<^sub>d, \<Xi> \<turnstile> VSum tag' v :v instantiate \<tau>s (TSum ts)"
       using x_is typing_x1 \<gamma>_matches_\<Gamma>1 v_sem_case_nm.hyps(2) v_sem_case_nm.prems
       by fastforce
-    then have "\<Xi> \<turnstile> VSum tag' v :v TSum (tagged_list_update tag (instantiate \<tau>s ta, Checked) (map (\<lambda>(c, t, b). (c, instantiate \<tau>s t, b)) ts))"
+    then have "\<Xi>\<^sub>d, \<Xi> \<turnstile> VSum tag' v :v TSum (tagged_list_update tag (instantiate \<tau>s ta, Checked) (map (\<lambda>(c, t, b). (c, instantiate \<tau>s t, b)) ts))"
       using v_sem_case_nm.hyps(3) image_iff ta_in_ts
       by (fastforce intro!: sum_downcast)
-    then have "\<Xi> \<turnstile> VSum tag' v :v instantiate \<tau>s (TSum (tagged_list_update tag (ta, Checked) ts))"
+    then have "\<Xi>\<^sub>d, \<Xi> \<turnstile> VSum tag' v :v instantiate \<tau>s (TSum (tagged_list_update tag (ta, Checked) ts))"
       by (simp add: tagged_list_update_map_over2[where f="\<lambda>(c, t, b). (c, instantiate \<tau>s t, b)" and g="\<lambda>(t,b). (instantiate \<tau>s t, b)"] case_prod_beta)
-    then show "\<Xi> \<turnstile> n' :v instantiate \<tau>s \<tau>"
+    then show "\<Xi>\<^sub>d, \<Xi> \<turnstile> n' :v instantiate \<tau>s \<tau>"
       using v_sem_case_nm.prems v_sem_case_nm.hyps(5) \<gamma>_matches_\<Gamma>2 matches_cons
         n_is typing_x4
       by blast
   qed
 next
-  case (v_sem_esac \<xi> \<gamma> spec_a tag v)
+  case (v_sem_esac \<xi>\<^sub>d \<xi> \<gamma> spec_a tag v)
   then show ?case
   proof (cases e)
     case (Esac a)
@@ -935,24 +992,24 @@ next
 
     then obtain ts' tag'
       where esac_elims:
-        "\<Xi>, K, \<Gamma> \<turnstile> a : TSum ts'"
+        "\<Xi>\<^sub>d, \<Xi>, K, \<Gamma> \<turnstile> a : TSum ts'"
         "[(tag', \<tau>, Unchecked)] = filter ((=) Unchecked \<circ> snd \<circ> snd) ts'"
       using v_sem_esac.prems Esac
       by blast
 
-    have "\<Xi> \<turnstile> VSum tag v :v instantiate \<tau>s (TSum ts')"
+    have "\<Xi>\<^sub>d, \<Xi> \<turnstile> VSum tag v :v instantiate \<tau>s (TSum ts')"
       using v_sem_esac.hyps(2) v_sem_esac.prems esac_simps esac_elims
       by blast
     then obtain \<tau>'
       where ih_elims:
-        "\<Xi> \<turnstile> v :v instantiate \<tau>s \<tau>'"
+        "\<Xi>\<^sub>d, \<Xi> \<turnstile> v :v instantiate \<tau>s \<tau>'"
         "(tag, instantiate \<tau>s \<tau>', Unchecked) \<in> set (map (\<lambda>(c, t, b). (c, instantiate \<tau>s t, b)) ts')"
         "distinct (map fst ts')"
         "[] \<turnstile> instantiate \<tau>s (TSum ts') wellformed"
       by (force simp add: kinding_simps)
     then have "(tag, instantiate \<tau>s \<tau>', Unchecked) = (tag', instantiate \<tau>s \<tau>, Unchecked)"
       using esac_elims ih_elims by (fastforce simp add: filter_eq_singleton_iff2)
-    then show "\<Xi> \<turnstile> v :v instantiate \<tau>s \<tau>"
+    then show "\<Xi>\<^sub>d, \<Xi> \<turnstile> v :v instantiate \<tau>s \<tau>"
       using ih_elims by simp
   qed clarsimp+
 next case v_sem_let     then show ?case by ( case_tac e, simp_all
@@ -969,7 +1026,7 @@ next case v_sem_struct  then show ?case by ( case_tac e, simp_all
                                                               vval_typing_all_record [ where ts = "map f ts" for f ts
                                                                                      , simplified])
 next
-  case (v_sem_take \<xi> \<gamma> spec_x fs f' spec_y e')
+  case (v_sem_take \<xi>\<^sub>d \<xi> \<gamma> spec_x fs f' spec_y e')
   then show ?case
   proof (cases e)
     case (Take x f y)
@@ -982,31 +1039,31 @@ next
     obtain \<Gamma>1 \<Gamma>2 ts s n t k taken
       where typing_elims:
         "K \<turnstile> \<Gamma> \<leadsto> \<Gamma>1 | \<Gamma>2"
-        "\<Xi>, K, \<Gamma>1 \<turnstile> x : TRecord ts s"
+        "\<Xi>\<^sub>d, \<Xi>, K, \<Gamma>1 \<turnstile> x : TRecord ts s"
         "sigil_perm s \<noteq> Some ReadOnly"
         "f < length ts"
         "ts ! f = (n, t, Present)"
         "K \<turnstile> t :\<kappa> k"
         "S \<in> k \<or> taken = Taken"
-        "\<Xi>, K, Some t # Some (TRecord (ts[f := (n, t, taken)]) s) # \<Gamma>2 \<turnstile> y : \<tau>"
+        "\<Xi>\<^sub>d, \<Xi>, K, Some t # Some (TRecord (ts[f := (n, t, taken)]) s) # \<Gamma>2 \<turnstile> y : \<tau>"
       using v_sem_take.prems(1) spec_simps Take
       by blast
     then have matchsplit_lemmas:
-      "\<Xi> \<turnstile> \<gamma> matches instantiate_ctx \<tau>s \<Gamma>1"
-      "\<Xi> \<turnstile> \<gamma> matches instantiate_ctx \<tau>s \<Gamma>2"
+      "\<Xi>\<^sub>d, \<Xi> \<turnstile> \<gamma> matches instantiate_ctx \<tau>s \<Gamma>1"
+      "\<Xi>\<^sub>d, \<Xi> \<turnstile> \<gamma> matches instantiate_ctx \<tau>s \<Gamma>2"
       using matches_split2 v_sem_take.prems
       by blast+
     
-    have "\<Xi> \<turnstile> VRecord fs :v instantiate \<tau>s (TRecord ts s)"
+    have "\<Xi>\<^sub>d, \<Xi> \<turnstile> VRecord fs :v instantiate \<tau>s (TRecord ts s)"
       using v_sem_take.prems spec_simps typing_elims matchsplit_lemmas
       by (fastforce intro!: v_sem_take.hyps(2))
     moreover then have all_inst_ts:
-      "\<Xi> \<turnstile>* fs :vr map (\<lambda>(n, t, b). (n, instantiate \<tau>s t, b)) ts"
+      "\<Xi>\<^sub>d, \<Xi> \<turnstile>* fs :vr map (\<lambda>(n, t, b). (n, instantiate \<tau>s t, b)) ts"
       "distinct (map fst ts)"
       by (fastforce)+
     moreover then have "\<And>t' b'. distinct (map fst (ts[f := (n, t', b')]))"
       by (simp add: map_fst_update typing_elims)
-    ultimately have "\<Xi> \<turnstile> VRecord fs :v TRecord (map (\<lambda>(n, t, b). (n, instantiate \<tau>s t, b)) (ts[f := (n, t, taken)])) s"
+    ultimately have "\<Xi>\<^sub>d, \<Xi> \<turnstile> VRecord fs :v TRecord (map (\<lambda>(n, t, b). (n, instantiate \<tau>s t, b)) (ts[f := (n, t, taken)])) s"
       using typing_elims v_sem_take.prems
       by (fastforce simp add: map_update intro: substitutivity vval_typing_vval_typing_record.intros vval_typing_record_take)
     then show ?thesis
@@ -1014,7 +1071,7 @@ next
       by (fastforce intro!: v_sem_take.hyps(4) simp add: matches_Cons vval_typing_record_nth)
   qed simp+
 next
-  case (v_sem_put \<xi> \<gamma> x_spec fs ea_spec ea' f)
+  case (v_sem_put \<xi>\<^sub>d \<xi> \<gamma> x_spec fs ea_spec ea' f)
   
   then show ?case
   proof (case_tac e; clarsimp)
@@ -1027,28 +1084,28 @@ next
       where typingelims:
         "\<tau> = TRecord (ts[f := (n, t, Present)]) s"
         "K \<turnstile> \<Gamma> \<leadsto> \<Gamma>1 | \<Gamma>2"
-        "\<Xi>, K, \<Gamma>1 \<turnstile> x : TRecord ts s"
+        "\<Xi>\<^sub>d, \<Xi>, K, \<Gamma>1 \<turnstile> x : TRecord ts s"
         "sigil_perm s \<noteq> Some ReadOnly"
         "f < length ts"
         "ts ! f = (n, t, taken)"
         "K \<turnstile> t :\<kappa> k"
         "D \<in> k \<or> taken = Taken"
-        "\<Xi>, K, \<Gamma>2 \<turnstile> ea : t"
+        "\<Xi>\<^sub>d, \<Xi>, K, \<Gamma>2 \<turnstile> ea : t"
       using v_sem_put by blast
     
     have IHresults:
-      "\<Xi> \<turnstile> VRecord fs :v instantiate \<tau>s (TRecord ts s)"
-      "\<Xi> \<turnstile> ea' :v instantiate \<tau>s t"
+      "\<Xi>\<^sub>d, \<Xi> \<turnstile> VRecord fs :v instantiate \<tau>s (TRecord ts s)"
+      "\<Xi>\<^sub>d, \<Xi> \<turnstile> ea' :v instantiate \<tau>s t"
       using v_sem_put.prems assms1 typingelims matches_split
       by (fast intro: v_sem_put.hyps(2,4))+
     then obtain ts' s'
       where instvrecordelims:
         "instantiate \<tau>s (TRecord ts s) = TRecord ts' s'"
-        "\<Xi> \<turnstile>* fs :vr ts'"
+        "\<Xi>\<^sub>d, \<Xi> \<turnstile>* fs :vr ts'"
         "distinct (map fst ts')"
       by blast
 
-    show "\<Xi> \<turnstile> VRecord (fs[f := ea']) :v instantiate \<tau>s \<tau>"
+    show "\<Xi>\<^sub>d, \<Xi> \<turnstile> VRecord (fs[f := ea']) :v instantiate \<tau>s \<tau>"
       using v_sem_put assms1 typingelims IHresults instvrecordelims
     proof (simp add: map_update, intro vval_typing_vval_typing_record.intros vval_typing_record_put)
       show "[] \<turnstile> instantiate \<tau>s t :\<kappa> k"
@@ -1066,33 +1123,35 @@ next case v_sem_split   then show ?case by ( case_tac e, simp_all
                                            , fastforce intro!: matches_cons
                                                        intro:  matches_split)
 
-next case (v_sem_app \<xi> \<gamma> x ea ts y a r e \<tau>s K \<tau> \<Gamma>)
+next case (v_sem_app \<xi>\<^sub>d \<xi> \<gamma> x ea ts y a r e \<tau>s K \<tau> \<Gamma>)
   obtain efun earg where e_def: "e = App efun earg"
       "x = specialise \<tau>s efun"
       "y = specialise \<tau>s earg"
     using v_sem_app by (cases e, auto)
 
-  obtain \<Gamma>1 \<Gamma>2 targ where app_elims:
+  obtain \<Gamma>1 \<Gamma>2 t targ where app_elims:
     "K \<turnstile> \<Gamma> \<leadsto> \<Gamma>1 | \<Gamma>2"
-    "\<Xi>, K, \<Gamma>1 \<turnstile> efun : TFun targ \<tau>"
-    "\<Xi>, K, \<Gamma>2 \<turnstile> earg : targ"
-    using v_sem_app e_def by blast
+    "t=  TFun targ \<tau> \<or>  t = TDFun targ \<tau>"
+    "\<Xi>\<^sub>d, \<Xi>, K, \<Gamma>1 \<turnstile> efun : t"
+    "\<Xi>\<^sub>d, \<Xi>, K, \<Gamma>2 \<turnstile> earg : targ"
+    using v_sem_app e_def by blast 
 
-  have vfun_ty: "\<Xi> \<turnstile> VFunction ea ts :v instantiate \<tau>s (TFun targ \<tau>)"
-    using app_elims e_def v_sem_app matches_split
-    by fast
+  have vfun_ty: "\<Xi>\<^sub>d, \<Xi> \<turnstile> VFunction ea ts :v instantiate \<tau>s (TFun targ \<tau>)"
+    using app_elims e_def v_sem_app matches_split 
+    by (smt instantiate.simps(6) type.distinct(69) value_sem.v_t_funE value_sem_axioms)
+   (* check this proof *)
 
-  have varg_ty: "\<Xi> \<turnstile> a :v instantiate \<tau>s targ"
-    using app_elims e_def v_sem_app matches_split
-    by fast
+  have varg_ty: "\<Xi>\<^sub>d, \<Xi> \<turnstile> a :v instantiate \<tau>s targ"
+    by (metis app_elims e_def v_sem_app matches_split)
+    
 
-  obtain Kfun t u where vfun_ty_elims: "\<Xi>, Kfun, [Some t] \<turnstile> ea : u"
+  obtain Kfun t u where vfun_ty_elims: "\<Xi>\<^sub>d, \<Xi>, Kfun, [Some t] \<turnstile> ea : u"
        "type_wellformed (length Kfun) t"
        "list_all2 (kinding []) ts Kfun"
        "[] \<turnstile> TFun (instantiate ts t) (instantiate ts u) \<sqsubseteq> TFun (instantiate \<tau>s targ) (instantiate \<tau>s \<tau>)"
     using vfun_ty by (auto elim: vval_typing.cases)
 
-  have vres_ty_sub: "\<Xi> \<turnstile> r :v instantiate ts u"
+  have vres_ty_sub: "\<Xi>\<^sub>d, \<Xi> \<turnstile> r :v instantiate ts u"
     using vfun_ty_elims v_sem_app(6)
     using matches_cons' matches_empty subtyping_simps(5) v_sem_app.prems(3) v_sem_app.prems(5) value_subtyping(1) varg_ty 
     by fastforce
@@ -1101,7 +1160,7 @@ next case (v_sem_app \<xi> \<gamma> x ea ts y a r e \<tau>s K \<tau> \<Gamma>)
     using app_elims e_def v_sem_app vfun_ty_elims vres_ty_sub
     by (metis subtyping_simps(5) value_subtyping(1))
 
-next case (v_sem_abs_app \<xi> \<gamma> x f ts y a r)
+next case (v_sem_abs_app \<xi>\<^sub>d \<xi> \<gamma> x f ts y a r)
   obtain efun earg where e_def: "e = App efun earg"
       "x = specialise \<tau>s efun"
       "y = specialise \<tau>s earg"
@@ -1109,15 +1168,15 @@ next case (v_sem_abs_app \<xi> \<gamma> x f ts y a r)
 
   obtain \<Gamma>1 \<Gamma>2 targ where app_elims:
     "K \<turnstile> \<Gamma> \<leadsto> \<Gamma>1 | \<Gamma>2"
-    "\<Xi>, K, \<Gamma>1 \<turnstile> efun : TFun targ \<tau>"
-    "\<Xi>, K, \<Gamma>2 \<turnstile> earg : targ"
-    using v_sem_abs_app e_def by blast
+    "\<Xi>\<^sub>d, \<Xi>, K, \<Gamma>1 \<turnstile> efun : TFun targ \<tau>"
+    "\<Xi>\<^sub>d, \<Xi>, K, \<Gamma>2 \<turnstile> earg : targ"
+    using v_sem_abs_app e_def  
 
-  have vafun_ty: "\<Xi> \<turnstile> VAFunction f ts :v instantiate \<tau>s (TFun targ \<tau>)"
+  have vafun_ty: "\<Xi>\<^sub>d, \<Xi> \<turnstile> VAFunction f ts :v instantiate \<tau>s (TFun targ \<tau>)"
     using app_elims e_def v_sem_abs_app matches_split
     by fast
 
-  have varg_ty: "\<Xi> \<turnstile> a :v instantiate \<tau>s targ"
+  have varg_ty: "\<Xi>\<^sub>d, \<Xi> \<turnstile> a :v instantiate \<tau>s targ"
     using app_elims e_def v_sem_abs_app matches_split
     by fast
 
@@ -1129,7 +1188,7 @@ next case (v_sem_abs_app \<xi> \<gamma> x f ts y a r)
       "[] \<turnstile> TFun (instantiate ts t) (instantiate ts u) \<sqsubseteq> TFun t' u'"
     using vafun_ty by (auto elim: vval_typing.cases)
 
-  have vres_ty_sub: "\<Xi> \<turnstile> r :v instantiate ts u"
+  have vres_ty_sub: "\<Xi>\<^sub>d, \<Xi> \<turnstile> r :v instantiate ts u"
     using vafun_ty_elims varg_ty v_sem_abs_app
     using subtyping_simps(5) value_subtyping(1)  instantiate.simps(5) proc_env_matches_abstract
     by metis
@@ -1145,7 +1204,7 @@ next case v_sem_all_cons  then show ?case by ( case_tac es, simp_all
                                              , fastforce simp: vval_typing_all_def
                                                          dest: matches_split)
 next
-  case (v_sem_promote \<Xi> \<xi> \<gamma> ea ea' t)
+  case (v_sem_promote \<Xi> \<xi>\<^sub>d \<xi> \<gamma> ea ea' t)
   then show ?case
     using value_subtyping(1) specialisation(1) typing_promoteE instantiate_ctx_nothing instantiate_nothing list.ctr_transfer(1) specialise_nothing
     by (metis)
@@ -1158,7 +1217,7 @@ qed
 lemma order_sum_list: "x \<in> set es \<Longrightarrow> x < Suc (sum_list es)"
   by (simp add: le_imp_less_Suc member_le_sum_list)
 
-function monoexpr :: "'f expr \<Rightarrow> ('f \<times> type list) expr" where
+function monoexpr :: "('f, 'g) expr \<Rightarrow> ('f \<times> type list) expr" where
   "monoexpr (AFun f ts)       = AFun (f, ts) []"
 | "monoexpr (Fun f ts)        = Fun (monoexpr (specialise ts f)) []"
 | "monoexpr (Var i)           = Var i"
@@ -1185,7 +1244,7 @@ function monoexpr :: "'f expr \<Rightarrow> ('f \<times> type list) expr" where
              by (case_tac x, auto)
 termination by (relation "measure expr_size", (simp add: order_sum_list)+)
 
-fun monoval :: "('f, 'a, 'b) vval \<Rightarrow> ('f \<times> type list, 'a, 'b) vval"
+fun monoval :: "('f, 'g, 'a, 'b) vval \<Rightarrow> ('f \<times> type list, 'a, 'b) vval"
 where "monoval (VPrim lit) = VPrim lit"
     | "monoval (VProduct t u) = VProduct (monoval t) (monoval u)"
     | "monoval (VSum name v) = VSum name (monoval v)"
@@ -1197,14 +1256,14 @@ where "monoval (VPrim lit) = VPrim lit"
     | "monoval VUnit = VUnit"
 
 
-definition monoprog :: "('f, 'a, 'b) vabsfuns \<Rightarrow> (('f \<times> type list), 'a, 'b) vabsfuns \<Rightarrow> bool"
+definition monoprog :: "('f, 'g, 'a, 'b) vabsfuns \<Rightarrow> (('f \<times> type list), 'a, 'b) vabsfuns \<Rightarrow> bool"
 where "monoprog \<xi> \<xi>' \<equiv> \<forall>f \<tau>s. (\<forall>v v'. \<xi> f v v' \<longleftrightarrow> \<xi>' (f, \<tau>s) (monoval v) (monoval v'))"
 
 lemma member_nth_map: "f < length fs \<Longrightarrow> \<xi>', map monoval \<gamma> \<turnstile> Member (monoexpr e) f \<Down> monoval (fs ! f) =  \<xi>' , map monoval \<gamma> \<turnstile> Member (monoexpr e) f \<Down> (map monoval fs) ! f"
 by (subst nth_map, simp_all)
 thm v_sem_prim
 
-lemma v_sem_prim': "\<xi> , \<gamma> \<turnstile>* as \<Down> as' \<Longrightarrow> eval_prim p as' = r \<Longrightarrow> \<xi> , \<gamma> \<turnstile> Prim p as \<Down> r"
+lemma v_sem_prim': "\<xi>\<^sub>d , \<xi> , \<gamma> \<turnstile>* as \<Down> as' \<Longrightarrow> eval_prim p as' = r \<Longrightarrow> \<xi>\<^sub>d , \<xi> , \<gamma> \<turnstile> Prim p as \<Down> r"
 by (force dest: sym intro: v_sem_prim)
 
 lemma monoval_vprim [simp]: "monoval \<circ> VPrim = VPrim" by (rule ext, simp)
@@ -1214,8 +1273,8 @@ assumes "\<xi> matches \<Xi>"
 and     "proc_ctx_wellformed \<Xi>"
 and     "\<Xi> \<turnstile> \<gamma> matches \<Gamma>"
 and     "monoprog \<xi> \<xi>'"
-shows   "\<xi>, \<gamma> \<turnstile> e \<Down> e' \<Longrightarrow>  \<Xi>, [], \<Gamma> \<turnstile> e : \<tau>    \<Longrightarrow> \<xi>', map monoval \<gamma> \<turnstile> monoexpr e \<Down> monoval e'"
- and     "\<xi>, \<gamma> \<turnstile>* es \<Down> es' \<Longrightarrow> \<Xi>, [], \<Gamma> \<turnstile>* es : \<tau>s \<Longrightarrow> \<xi>', map monoval \<gamma> \<turnstile>* map monoexpr es \<Down> map monoval es'"
+shows   "\<xi>\<^sub>d, \<xi>, \<gamma> \<turnstile> e \<Down> e' \<Longrightarrow>  \<Xi>, [], \<Gamma> \<turnstile> e : \<tau>    \<Longrightarrow> \<xi>', map monoval \<gamma> \<turnstile> monoexpr e \<Down> monoval e'"
+ and     "\<xi>\<^sub>d, \<xi>, \<gamma> \<turnstile>* es \<Down> es' \<Longrightarrow> \<Xi>, [], \<Gamma> \<turnstile>* es : \<tau>s \<Longrightarrow> \<xi>', map monoval \<gamma> \<turnstile>* map monoexpr es \<Down> map monoval es'"
 using assms proof (induct \<xi> \<gamma> e e'
                       and \<xi> \<gamma> es es'
                arbitrary: \<tau> \<Gamma>
